Merge with Ky

concurrency/Cmm_op_proofs.thy
@@ -1,3 +1,4 @@
+(*<*)
 theory Cmm_op_proofs
 
 imports
@@ -6,10 +7,11 @@ Main
 Cmm_master_lemmas
 Nondeterminism_lemmas  
 begin
+(*>*)
 
 section {* The axiomatic model *}
 
-abbreviation "sublanguage \<equiv> true_condition"
+abbreviation "sublanguage \<equiv> with_consume_condition"
 abbreviation "memory_model \<equiv> standard_memory_model"
 abbreviation "axBehaviour \<equiv> standard_behaviour"
 abbreviation "axUndefined \<equiv> locks_only_undefined_behaviour_alt"
@@ -19,7 +21,7 @@ abbreviation "getVse \<equiv> with_consume_vse"
 abbreviation "axConsistent ex \<equiv> apply_tree standard_consistent_execution ex"
 abbreviation "axConsistentAlt pre wit \<equiv> axConsistent (pre, wit, getRelations pre wit)"
 
-lemmas sublanguage_def = true_condition_def
+lemmas sublanguage_def = with_consume_condition_def
 lemmas memory_model_def = with_consume_memory_model_def
 lemmas axBehaviour_def = standard_behaviour_def
 lemmas axUndefined_def = locks_only_undefined_behaviour_alt_def
@@ -36,11 +38,7 @@ lemmas getRelations_simp = standard_relations_simp
 
 section {* The simplified axiomatic model *}
 
-abbreviation "axsimpConsistent ex \<equiv> apply_tree axsimpConsistentExecution ex"
-abbreviation "axsimpConsistentAlt pre wit \<equiv> axsimpConsistent (pre, wit, getRelations pre wit)"
-
-lemmas axsimpConsistent_def = axsimpConsistentExecution_def
-lemmas axsimpConsistentAlt_def = axsimpConsistent_def
+subsection {* well_formed_threads_opsem *}
 
 lemma rel_list_well_formed_threads_opsem [simp]:
   assumes "rel \<noteq> []"
@@ -83,6 +81,38 @@ using assms
 unfolding well_formed_threads_opsem_eq
 by auto
 
+subsection {* axsimpConsistent *}
+
+abbreviation "axsimpConsistent ex \<equiv> apply_tree axsimpConsistentExecution ex"
+abbreviation "axsimpConsistentAlt pre wit \<equiv> axsimpConsistent (pre, wit, getRelations pre wit)"
+
+lemmas axsimpConsistent_def = axsimpConsistentExecution_def
+lemmas axsimpConsistentAlt_def = axsimpConsistent_def
+
+lemma axsimpConsistentI [intro?]: 
+  assumes "assumptions (pre, wit, [])"
+      and "tot_empty (pre, wit, [])"
+      and "well_formed_threads_opsem (pre, wit, [])"
+      and "well_formed_rf (pre, wit, [])"
+      and "locks_only_consistent_locks (pre, wit, [])"
+      and "locks_only_consistent_lo (pre, wit, [(''hb'', getHb pre wit)])"
+      and "consistent_mo (pre, wit, [])"
+      and "sc_accesses_consistent_sc (pre, wit, [(''hb'', getHb pre wit)])"
+      and "sc_fenced_sc_fences_heeded (pre, wit, [])"
+      and "consistent_hb (pre, wit, [(''hb'', getHb pre wit)])"
+      and "det_read_alt (pre, wit, [(''hb'', getHb pre wit)])"
+      and "consistent_non_atomic_rf (pre, wit, [(''hb'', getHb pre wit), 
+                                                (''vse'', getVse pre wit)])"
+      and "consistent_atomic_rf (pre, wit, [(''hb'', getHb pre wit)])"
+      and "coherent_memory_use (pre, wit, [(''hb'', getHb pre wit)])"
+      and "rmw_atomicity (pre, wit, [])"
+      and "sc_accesses_sc_reads_restricted (pre, wit, [(''hb'', getHb pre wit)])"
+  shows   "axsimpConsistentAlt pre wit"
+using assms
+unfolding axsimpConsistent_def
+          memory_model_def
+by simp_all
+
 lemma axsimpConsistentE [elim]: 
   assumes "axsimpConsistentAlt pre wit"
   obtains "assumptions (pre, wit, [])"
@@ -121,6 +151,8 @@ unfolding axsimpConsistent_def
           ex_def 
 by simp metis
 
+subsection {* axsimpMemoryModel *}
+
 lemma axsimpMemoryModel_simps [simp]:
   shows "consistent axsimpMemoryModel = axsimpConsistentExecution"
         "relation_calculation axsimpMemoryModel = standard_relations"
@@ -147,13 +179,14 @@ qed *)
 
 section {* The incremental model *}
 
+subsection {* Simplifications *}
+
 abbreviation "hbMinusAlt pre wit \<equiv> hbMinus (pre,wit, getRelations pre wit)"
 abbreviation "incComAlt pre wit \<equiv> incCom (pre,wit, getRelations pre wit)"
+abbreviation "incCommittedSet s \<equiv> set (incCommitted s)"
 
 lemmas hbMinusAlt_def = hbMinus.simps
 lemmas incComAlt_def = incCom.simps
-
-subsection {* Simplifications *}
 
 lemma incPreRestrict_simps [simp]:
   shows "actions0 (preRestrict pre actions) = actions0 pre \<inter> actions "
@@ -234,7 +267,7 @@ by auto
 
 lemma initialState_simps [simp]:
   shows "incWit (incInitialState pre) = empty_witness"
-        "incCommitted (incInitialState pre) = {}"
+        "incCommitted (incInitialState pre) = []"
 unfolding incInitialState_def
 by simp_all
 
@@ -549,7 +582,7 @@ subsubsection {* Empty hb *}
 (* Empty hb in the with_consume fragment *)
 
 lemma sw_asw_empty [simp]:
-  shows "sw_asw (preRestrict pre {}) empty_witness = {}"
+  shows "sw_asw (preRestrict pre {}) = {}"
 unfolding sw_asw_def
 by simp
 
@@ -1091,10 +1124,10 @@ unfolding release_sequence_set_alt_def
 by auto
 
 lemma final_sw_asw:
-  assumes "(a, b) \<in> sw_asw pre wit"
+  assumes "(a, b) \<in> sw_asw pre"
       and "a \<in> actions" 
       and "b \<in> actions"
-  shows   "(a, b) \<in> sw_asw (preRestrict pre actions) (incWitRestrict wit actions)"
+  shows   "(a, b) \<in> sw_asw (preRestrict pre actions)"
 using assms
 unfolding sw_asw_def
 by auto
@@ -2084,7 +2117,7 @@ proof -
     using assms incPreRestrict_sbasw_subset
     unfolding well_formed_threads.simps
     unfolding blocking_observed_def
-              Cmm_master.inj_on_def
+              Cmm_csem.inj_on_def
               threadwise_def
               interthread_def
               isStrictPartialOrder_def
@@ -2305,12 +2338,13 @@ by simp
 lemma incTraceConsistency: 
   assumes "incTrace pre r s"
           "r = incInitialState pre"
-  shows   "  axsimpConsistentAlt (preRestrict pre (incCommitted s)) (incWit s)
-           \<and> well_formed_threads_opsem (pre, empty_witness, [])"
+  shows   "  axsimpConsistentAlt (preRestrict pre (incCommittedSet s)) (incWit s)
+           \<and> well_formed_threads_opsem (pre, empty_witness, [])
+           \<and> incCommittedSet s \<subseteq> actions0 pre"
 using assms 
 proof induct
   case incStep
-  thus ?case unfolding incStep_def Let_def by auto
+  thus ?case unfolding incStep_def incToEx_def Let_def by auto
 qed simp
 
 lemma incConsistentSoundness:
@@ -2321,8 +2355,9 @@ proof -
   assume "incConsistent (pre, wit, getRelations pre wit)"
   then obtain s where trace: "incTrace pre (incInitialState pre) s"
                   and   wit: "incWit s = wit"
-                  and   com: "incCommitted s = actions0 pre"
-    unfolding incConsistent.simps by auto
+                  and   com: "incCommittedSet s = actions0 pre"
+    unfolding incConsistent_def consistencyFromTrace.simps
+    by auto
   thus "axsimpConsistent (pre, wit, getRelations pre wit)" 
     using incTraceConsistency[OF trace] preRestrict_id wit
     by metis
@@ -2337,14 +2372,8 @@ lemma existenceIncTrace:
       and downclosed: "downclosed actions (incComAlt pre wit)"
   shows   "\<exists> s. incTrace pre (incInitialState pre) s \<and> 
                 incWit s = incWitRestrict wit actions \<and> 
-                incCommitted s = actions"
-proof (rule finite_downclosedsubset_induct[where R="(incComAlt pre wit)" and B="actions0 pre"])
-  show "finite actions" using finite .
-next
-  show "actions \<subseteq> actions0 pre" using universe .
-next
-  show "downclosed actions (incComAlt pre wit)" using downclosed .
-next
+                incCommittedSet s = actions"
+proof (rule finite_downclosedsubset_induct[OF finite universe downclosed])
   show "acyclic (incComAlt pre wit)"
     using opsemOrder_isStrictPartialOrder[OF cons]
     unfolding isStrictPartialOrder_def acyclic_def irrefl_def
@@ -2356,7 +2385,7 @@ next
     by (cases "wit = empty_witness") simp_all
   thus "\<exists>s.   incTrace pre (incInitialState pre) s 
             \<and> incWit s = incWitRestrict wit {} 
-            \<and> incCommitted s = {}"
+            \<and> incCommittedSet s = {}"
     using incReflexive by (intro exI[where x="incInitialState pre"]) simp
 next
   fix a :: action
@@ -2368,19 +2397,19 @@ next
      and max:         "\<forall>b\<in>actions. (a, b) \<notin> incComAlt pre wit"
      and IH:          "\<exists>s. incTrace pre (incInitialState pre) s \<and> 
                            incWit s = incWitRestrict wit actions \<and> 
-                           incCommitted s = actions"
+                           incCommittedSet s = actions"
   obtain s where trace:     "incTrace pre (incInitialState pre) s" 
              and witness:   "incWit s = incWitRestrict wit actions"
-             and committed: "incCommitted s = actions" using IH by blast
+             and committed: "incCommittedSet s = actions" using IH by blast
 
   let ?actions' = "insert a actions"
   let ?pre'     = "preRestrict pre ?actions'"
   let ?wit'     = "incWitRestrict wit ?actions'"
   let ?s' = "\<lparr> incWit=?wit', 
-               incCommitted=?actions'\<rparr>"
+               incCommitted=a#(incCommitted s)\<rparr>"
   have downclosed_mo: "downclosed ?actions' (mo wit)"
     using downclosed' unfolding incComAlt_def by auto
-  have inOpsemOrder: "respectsCom (actions0 pre) actions (incComAlt ?pre' (incWit ?s')) a"
+  have inOpsemOrder: "respectsCom (actions0 pre) (incCommitted s) (incComAlt ?pre' (incWit ?s')) a"
     unfolding respectsCom_def
     proof auto
       fix b
@@ -2395,30 +2424,33 @@ next
         using opsemOrder_isStrictPartialOrder[OF cons]
         unfolding isStrictPartialOrder_def irrefl_def
         by auto
-      thus "b \<in> actions"
-        using downclosed' ba_in_rel unfolding downclosed_def by auto
+      thus "b \<in> incCommittedSet s"
+        using downclosed' ba_in_rel committed 
+        unfolding downclosed_def 
+        by auto
     next
       fix b
       (* TODO: fix opsemOrder *)
       assume "b \<in> actions0 pre"
-             "b \<in> actions"
+             "b \<in> incCommittedSet s"
              "(a, b) \<in> incComAlt ?pre' ?wit'"
       hence ba_in_rel: "(a, b) \<in> incComAlt pre wit"
         using opsemOrderIsMonotonic downclosed_mo
         unfolding hbCalcIsMonotonic_def
         by auto
-      thus False using max `b \<in> actions` by metis 
+      thus False using max `b \<in> incCommittedSet s` committed  by metis 
     qed
   have "axsimpConsistentAlt ?pre' ?wit'"
     using cons downclosed' axsimpConsistent_restriction by metis
   hence "incStep pre s ?s' a"
-    unfolding incStep_def Let_def 
+    unfolding incStep_def Let_def incToEx_def
     using committed `a \<notin> actions` `a \<in> actions0 pre` witness inOpsemOrder
     by auto
   hence "incTrace pre (incInitialState pre) ?s'" using incStep trace by smt
   thus "\<exists>s'. incTrace pre (incInitialState pre) s' \<and> 
              incWit s' = incWitRestrict wit ?actions' \<and> 
-             incCommitted s' = ?actions'"
+             incCommittedSet s' = ?actions'"
+    using committed
     by (intro exI[where x="?s'"]) simp
 qed
 
@@ -2462,13 +2494,22 @@ proof -
     using cons by auto
   obtain s where "incTrace pre (incInitialState pre) s"
                            "incWit s = incWitRestrict wit (actions0 pre)"
-                           "incCommitted s = (actions0 pre)"
+                           "incCommittedSet s = (actions0 pre)"
     using existenceIncTrace[OF cons finite _ downclosed]
     by auto
   thus ?thesis
-    unfolding incConsistent.simps using wit_restrict by auto
+    unfolding incConsistent_def consistencyFromTrace.simps
+    using wit_restrict
+    by auto
 qed
 
+subsection {* Equivalence *}
+
+corollary incConsistentEquivalence:
+  shows "  incConsistent (pre, wit, getRelations pre wit)
+         = axsimpConsistent (pre, wit, getRelations pre wit)"
+using incConsistentSoundness incConsistentCompleteness
+by metis
 
 
 section {* The monadic model *}
@@ -2477,96 +2518,188 @@ subsubsection {* monInvariant *}
 
 definition monInvariant :: "pre_execution \<Rightarrow> incState \<Rightarrow> bool" where
   "monInvariant pre s \<equiv> 
-        axsimpConsistentAlt (preRestrict pre (incCommitted s)) (incWit s)
+        axsimpConsistentAlt (preRestrict pre (incCommittedSet s)) (incWit s)
       \<and> well_formed_threads_opsem (pre, empty_witness, [])
-      \<and> incCommitted s \<subseteq> actions0 pre"
+      \<and> incCommittedSet s \<subseteq> actions0 pre"
 
 lemma monInvariantE [elim]:
   assumes "monInvariant pre s"
-  obtains "axsimpConsistentAlt (preRestrict pre (incCommitted s)) (incWit s)"
+  obtains "axsimpConsistentAlt (preRestrict pre (incCommittedSet s)) (incWit s)"
       and "well_formed_threads_opsem (pre, empty_witness, [])"
-      and "incCommitted s \<subseteq> actions0 pre"
+      and "incCommittedSet s \<subseteq> actions0 pre"
 using assms
 unfolding monInvariant_def
 by simp
 
-lemma monInvariantE_incCommittedFinite [elim]:
-  assumes "monInvariant pre s"
-  obtains "finite (incCommitted s)"
-proof -
-  have "incCommitted s \<subseteq> actions0 pre" "finite (actions0 pre)"
-    using assms by auto
-  thus ?thesis using that finite_subset by auto
-qed
-
 subsection {* Elims of auxiliaries *}
 
+subsubsection {* list comprehensions *}
+
+lemma setFoldr_filter_simp [simp]:
+  shows "  set (foldr (\<lambda>e x2. if P e then f e # x2 else x2) l [])
+         = f ` {e. e \<in> set l \<and> P e}"
+by (induct l) auto
+
+lemma setFoldr_map_simp [simp]:
+  shows "  set (foldr (\<lambda>b. op # (f b)) l [])
+         = f ` (set l)"
+by (induct l) auto
+
+subsubsection {* sameLocWrites *}
+
+abbreviation "sameLocWritesSet actions a \<equiv> set (sameLocWrites actions a)"
+
+lemmas sameLocWritesSet_def = sameLocWrites_def
+
 lemma sameLocWritesE [elim]:
-  assumes "x \<in> sameLocWrites actions a"
-  obtains "x \<in> actions" "is_write x" "loc_of x = loc_of a"
+  assumes "x \<in> set (sameLocWrites actions a)"
+  obtains "x \<in> set actions" "is_write x" "loc_of x = loc_of a"
 using assms
 unfolding sameLocWrites_def
 by auto
 
-lemma sameLocWrites_finite:
-  assumes "finite actions"
-  obtains "finite (sameLocWrites actions a)"
-using assms
-unfolding sameLocWrites_def
-by auto
+lemma sameLocInMo:
+  assumes sameLoc:    "w \<in> sameLocWritesSet committed a"
+      and cons2:      "axsimpConsistentAlt pre wit"
+      and committed:  "actions0 pre = insert a (set committed)"
+      and downclosed: "downclosed (set committed) (mo wit)"
+      and a:          "is_at_atomic_location (lk pre) a"
+                      "is_write a"
+                      "a \<in> actions0 pre"
+                      "a \<notin> set committed"
+  shows   "(w, a) \<in> mo wit"
+proof -  
+  have bc: "loc_of w = loc_of a" 
+           "is_write w" 
+           "w \<in> set committed"
+    using sameLoc by auto
+  hence bc2: "w \<noteq> a" 
+             "is_write a" 
+             "is_at_atomic_location (lk pre) a"
+             "w \<in> actions0 pre"
+             "a \<in> actions0 pre"
+             "a \<notin> set committed"
+    using a committed by auto
+  hence "(a, w) \<notin> mo wit"
+    using downclosed bc by (auto elim: downclosedE)
+  thus "(w, a) \<in> mo wit" 
+    using cons2 bc bc2 by (auto elim: consistent_moE_inv)
+qed
+
+subsubsection {* sameLocLocksUnlocks *}
+
+abbreviation "sameLocLocksUnlocksSet actions a \<equiv> set (sameLocLocksUnlocks actions a)"
+
+lemmas sameLocLocksUnlocksSet_def = sameLocLocksUnlocks_def
 
 lemma sameLocLocksUnlocksE [elim]:
-  assumes "x \<in> sameLocLocksUnlocks actions a"
-  obtains "x \<in> actions" "is_lock x \<or> is_unlock x" "loc_of x = loc_of a"
+  assumes "x \<in> set (sameLocLocksUnlocks actions a)"
+  obtains "x \<in> set actions" "is_lock x \<or> is_unlock x" "loc_of x = loc_of a"
 using assms
 unfolding sameLocLocksUnlocks_def
 by auto
 
+subsubsection {* scActions *}
+
+abbreviation "scActionsSet actions \<equiv> set (scActions actions)"
+
+lemmas scActionsSet_def = scActions_def
+
 lemma scActionsE [elim]:
-  assumes "x \<in> scActions actions"
-  obtains "x \<in> actions" "is_seq_cst x"
+  assumes "x \<in> set (scActions actions)"
+  obtains "x \<in> set actions" "is_seq_cst x"
 using assms
 unfolding scActions_def
 by auto
 
+subsubsection {* checkValuesAreEqual *}
+
+lemmas checkValuesAreEqual.simps [simp]
+
+lemma checkValuesAreEqual_simp [simp]:
+  shows "() [\<in>] checkValuesAreEqual b = (b = None \<or> (\<exists>a. b = Some (a, a)))"
+by (cases b) auto
+
+subsubsection {* addToTransitiveOrder *}
+
+lemma addToTransitiveOrderE [elim?]:
+  assumes "rel' [\<in>] addToTransitiveOrder domain a rel"
+  obtains y where "y \<in> set domain"
+                  "rel' = insert (y, a) 
+                                 (   rel 
+                                   \<union> (\<lambda>c. (c, a)) ` {c \<in> set domain. (c, y) \<in> rel}
+                                   \<union> Pair a ` {c \<in> set domain. (y, c) \<in> rel}
+                                 )"
+        | "rel' = rel \<union> Pair a ` set domain"
+using assms
+unfolding addToTransitiveOrder_def
+by auto
+
+lemma addToTransitiveOrderE_elem [elim?]:
+  assumes "rel' [\<in>] addToTransitiveOrder domain a rel"
+      and "(x, y) \<in> rel'"
+  obtains "(x, y) \<in> rel"
+        | "x = a" "y \<in> set domain"
+        | "y = a" "x \<in> set domain"
+using assms
+unfolding addToTransitiveOrder_def
+by auto
+
+(*
+lemma addToTransitiveOrderE_elem2 [elim?]:
+  assumes "rel' [\<in>] addToTransitiveOrder domain a rel"
+      and "(x, y) \<in> rel"
+  obtains "(x, y) \<in> rel'"
+using assms
+unfolding addToTransitiveOrder_def
+by auto
+*)
+
 subsection {* Elims of relation constructions *}
+
+subsubsection {* mo *}
 
 lemma monAddToMoE [elim?]:
   assumes step: "rel [\<in>] monAddToMo pre a s"
       and inv:  "monInvariant pre s"
-  obtains "rel = mo (incWit s) \<union> (\<lambda>b. (b, a)) ` sameLocWrites (incCommitted s) a"
+  obtains "rel = mo (incWit s) \<union> (\<lambda>b. (b, a)) ` sameLocWritesSet (incCommitted s) a"
 using assms
-unfolding monAddToMo_def Let_def
+unfolding monAddToMo_def Let_def 
 by auto
 
+subsubsection {* rf *}
+
 lemma auxAddPairToRfE [elim]: 
-  assumes step: "(rel', v) [\<in>] auxAddPairToRf rel w r eq"
-  obtains v_w v_r where "rel' = insert (w, r) rel"
-                        "v = Some (v_w, v_r)"
-                        "value_written_by w = Some v_w"
-                        "value_read_by r = Some v_r"
-                        "eq v_w v_r"
+  assumes step: "(rel', v_w, v_r) [\<in>] auxAddPairToRf rel w r "
+  obtains "rel' = insert (w, r) rel"
+          "value_written_by w = Some v_w"
+          "value_read_by r = Some v_r"
 using assms
 unfolding auxAddPairToRf_def
 apply (cases "value_written_by w", auto)
 by (cases "value_read_by r", auto)
 
 lemma auxAddToRfLoadE [elim?]:
-  assumes step: "(rel, v) [\<in>] auxAddToRfLoad pre a s eq"
-      and inv:  "monInvariant pre s"
-  obtains w where "w \<in> sameLocWrites (incCommitted s) a" 
-                  "(rel, v) [\<in>] auxAddPairToRf (rf (incWit s)) w a eq"
+  assumes step: "(rel, v) [\<in>] auxAddToRfLoad pre a s"
+  obtains w v_w v_r where "w \<in> sameLocWritesSet (incCommitted s) a" 
+                          "(rel, v_w, v_r) [\<in>] auxAddPairToRf (rf (incWit s)) w a"
+                          "v = Some (v_w, v_r)"
         | "rel = rf (incWit s)"
-proof (cases "rel = rf (incWit s)")
+          "v = None"
+proof (cases "v = None")
   case True
-  thus ?thesis using that by metis
+  hence "rel = rf (incWit s)"
+    using step 
+    unfolding auxAddToRfLoad_def
+    by auto
+  thus ?thesis using True that by metis
 next
   case False
-  have "finite (sameLocWrites (incCommitted s) a)"
-    using inv sameLocWrites_finite by auto
-  then obtain w where w: "w \<in> sameLocWrites (incCommitted s) a"
-                         "(rel, v) [\<in>] auxAddPairToRf (rf (incWit s)) w a eq"
-    using step False
+  then obtain w v_w v_r 
+        where w: "w \<in> sameLocWritesSet (incCommitted s) a"
+                 "(rel, v_w, v_r) [\<in>] auxAddPairToRf (rf (incWit s)) w a"
+                 "v = Some (v_w, v_r)"
+    using step 
     unfolding auxAddToRfLoad_def
     by auto
   thus ?thesis using w that by auto
@@ -2574,62 +2707,120 @@ qed
 
 lemma monAddToRfLoadE [elim?]:
   assumes step: "rel [\<in>] monAddToRfLoad pre a s"
-      and inv:  "monInvariant pre s"
-  obtains w v where "w \<in> sameLocWrites (incCommitted s) a" 
-                    "(rel, v) [\<in>] auxAddPairToRf (rf (incWit s)) w a op ="
+  obtains w v where "w \<in> sameLocWritesSet (incCommitted s) a" 
+                    "(rel, v, v) [\<in>] auxAddPairToRf (rf (incWit s)) w a"
         | "rel = rf (incWit s)"
 proof -
-  obtain v where v: "(rel, v) [\<in>] auxAddToRfLoad pre a s op ="
+  obtain vs where vs: "(rel, vs) [\<in>] auxAddToRfLoad pre a s"
+              and eq: "() [\<in>] checkValuesAreEqual vs"
     using step
     unfolding monAddToRfLoad_def
     by auto
   thus ?thesis
-    using that auxAddToRfLoadE[OF v inv]
-    by (cases "rel = rf (incWit s)") metis+
+    proof (cases "vs = None")
+      case True
+      hence "rel = rf (incWit s)"
+        using that auxAddToRfLoadE[OF vs]
+        by auto
+      thus ?thesis using that by metis
+    next
+      case False
+      then obtain w v_w v_r 
+            where w: "w \<in> sameLocWritesSet (incCommitted s) a" 
+                     "(rel, v_w, v_r) [\<in>] auxAddPairToRf (rf (incWit s)) w a"
+                     "vs = Some (v_w, v_r)"
+        using auxAddToRfLoadE[OF vs] by auto
+      hence "v_w = v_r" using eq by auto
+      thus ?thesis using that w by auto
+    qed
 qed
 
 lemma auxAddToRfRmwE [elim?]:
-  assumes step: "(rel, v) [\<in>] auxAddToRfRmw pre a s eq"
-      and inv:  "monInvariant pre s"
-  obtains w where "w \<in> sameLocWrites (incCommitted s) a"
-                  "\<forall>w' \<in> sameLocWrites (incCommitted s) a. (w, w') \<notin> mo (incWit s)"
-                  "(rel, v) [\<in>] auxAddPairToRf (rf (incWit s)) w a eq"
-        | "sameLocWrites (incCommitted s) a = {}"
+  assumes step: "(rel, v) [\<in>] auxAddToRfRmw pre a s"
+  obtains w v_w v_r where "w \<in> sameLocWritesSet (incCommitted s) a"
+                          "\<forall>w' \<in> sameLocWritesSet (incCommitted s) a. (w, w') \<notin> mo (incWit s)"
+                          "(rel, v_w, v_r) [\<in>] auxAddPairToRf (rf (incWit s)) w a"
+                          "v = Some (v_w, v_r)"
+        | "sameLocWrites (incCommitted s) a = []"
           "rel = rf (incWit s)"
-proof (cases "sameLocWrites (incCommitted s) a = {}")
+          "v = None"
+proof (cases "sameLocWrites (incCommitted s) a = []")
   case True
   thus ?thesis 
     using step that unfolding auxAddToRfRmw_def by auto
 next
   case False
-  have "finite (sameLocWrites (incCommitted s) a)"
-    using inv sameLocWrites_finite by auto
-  then obtain w where w: "w \<in> sameLocWrites (incCommitted s) a"
-                         "\<forall>w' \<in> sameLocWrites (incCommitted s) a. (w, w') \<notin> mo (incWit s)"
-                         "(rel, v) [\<in>] auxAddPairToRf (rf (incWit s)) w a eq"
-    using step False
+  then obtain w v_w v_r 
+        where w: "w \<in> sameLocWritesSet (incCommitted s) a"
+                 "\<forall>w' \<in> sameLocWritesSet (incCommitted s) a. (w, w') \<notin> mo (incWit s)"
+                 "(rel, v_w, v_r) [\<in>] auxAddPairToRf (rf (incWit s)) w a"
+                 "v = Some (v_w, v_r)"
+    using step 
     unfolding auxAddToRfRmw_def Let_def
     by auto
-  thus ?thesis using w that by auto
+  thus ?thesis using w that by metis
 qed
 
 lemma monAddToRfRmwE [elim?]:
   assumes step: "rel [\<in>] monAddToRfRmw pre a s"
-      and inv:  "monInvariant pre s"
-  obtains w v where "w \<in> sameLocWrites (incCommitted s) a" 
-                    "\<forall>w' \<in> sameLocWrites (incCommitted s) a. (w, w') \<notin> mo (incWit s)"
-                    "(rel, v) [\<in>] auxAddPairToRf (rf (incWit s)) w a op ="
-        | "sameLocWrites (incCommitted s) a = {}"
+  obtains w v where "w \<in> sameLocWritesSet (incCommitted s) a" 
+                    "\<forall>w' \<in> sameLocWritesSet (incCommitted s) a. (w, w') \<notin> mo (incWit s)"
+                    "(rel, v, v) [\<in>] auxAddPairToRf (rf (incWit s)) w a"
+        | "sameLocWrites (incCommitted s) a = []"
           "rel = rf (incWit s)"
 proof -
-  obtain v where v: "(rel, v) [\<in>] auxAddToRfRmw pre a s op ="
+  obtain vs where vs: "(rel, vs) [\<in>] auxAddToRfRmw pre a s"
+              and eq: "() [\<in>] checkValuesAreEqual vs"
     using step
     unfolding monAddToRfRmw_def
     by auto
   thus ?thesis
-    using that auxAddToRfRmwE[OF v inv]
-    by (cases "rel = rf (incWit s)") metis+
+    proof (cases "vs = None")
+      case True
+      hence "rel = rf (incWit s)" 
+            "sameLocWrites (incCommitted s) a = []"
+        using auxAddToRfRmwE[OF vs]
+        by auto
+      thus ?thesis using that by metis
+    next
+      case False
+      then obtain w v_w v_r 
+            where w: "w \<in> sameLocWritesSet (incCommitted s) a" 
+                     "\<forall>w' \<in> sameLocWritesSet (incCommitted s) a. (w, w') \<notin> mo (incWit s)"
+                     "(rel, v_w, v_r) [\<in>] auxAddPairToRf (rf (incWit s)) w a"
+                     "vs = Some (v_w, v_r)"
+        using auxAddToRfRmwE[OF vs] by auto
+      hence "v_w = v_r" using eq by auto
+      thus ?thesis using that w by auto
+    qed
 qed
+
+subsubsection {* sc *}
+
+subsubsection {* lo *}
+
+lemma monAddToLoE [elim?]:
+  assumes "rel' [\<in>] monAddToLo pre a s"
+  obtains y where "y \<in> sameLocLocksUnlocksSet (incCommitted s) a"
+                  "rel' = insert (y, a) 
+                                 (   lo (incWit s) 
+                                   \<union> (\<lambda>c. (c, a)) ` {c \<in> sameLocLocksUnlocksSet (incCommitted s) a. (c, y) \<in> lo (incWit s)}
+                                   \<union> Pair a ` {c \<in> sameLocLocksUnlocksSet (incCommitted s) a. (y, c) \<in> lo (incWit s)}
+                                 )"
+        | "rel' = lo (incWit s) \<union> Pair a ` (sameLocLocksUnlocksSet (incCommitted s) a)"
+using assms
+unfolding monAddToLo_def
+by (elim addToTransitiveOrderE) auto
+
+lemma monAddToLoE_elem [elim?]:
+  assumes "rel' [\<in>] monAddToLo pre a s"
+      and "(x, y) \<in> rel'"
+  obtains "(x, y) \<in> lo (incWit s)"
+        | "x = a" "y \<in> sameLocLocksUnlocksSet (incCommitted s) a"
+        | "y = a" "x \<in> sameLocLocksUnlocksSet (incCommitted s) a"
+using assms
+unfolding monAddToLo_def
+by (elim addToTransitiveOrderE_elem) auto
 
 subsection {* Elims of monStep *}
 
@@ -2637,14 +2828,14 @@ lemma monStepE_action [elim]:
   assumes monStep:  "(a, s2) [\<in>] monStep pre s1"
       and inv:  "monInvariant pre s"
   obtains "a \<in> actions0 pre" 
-          "a \<in> incCommitted s2"
-          "a \<notin> incCommitted s1"
+          "a \<in> incCommittedSet s2"
+          "a \<notin> incCommittedSet s1"
 proof -
   have "finite (actions0 pre)"
     using inv by auto
   hence "a \<in> actions0 pre" 
-        "a \<in> incCommitted s2"
-        "a \<notin> incCommitted s1"
+        "a \<in> incCommittedSet s2"
+        "a \<notin> incCommittedSet s1"
     using monStep
     unfolding monStep_def Let_def
     by auto
@@ -2653,19 +2844,19 @@ qed
 
 lemma monStepE_committed [elim]:
   assumes monStep:  "(a, s2) [\<in>] monStep pre s1"
-  obtains "incCommitted s2 = insert a (incCommitted s1)"
+  obtains "incCommitted s2 = a#(incCommitted s1)"
 using monStep
 unfolding monStep_def Let_def
 by auto
 
 lemmas monPerformActions_def = 
+  monPerformAction_def
   monPerformLock_def
   monPerformUnlock_def
   monPerformLoad_def
   monPerformStore_def
   monPerformRmw_def
   monPerformFence_def
-  monPerformBlocked_rmw_def
 
 subsubsection {* rf *}
 
@@ -2680,20 +2871,19 @@ by (cases a) auto
 
 lemma monStepE_rf2 [elim?]:
   assumes monStep: "(a, s2) [\<in>] monStep pre s1"
-      and inv:     "monInvariant pre s1"
   obtains w where "rf (incWit s2) = insert (w, a) (rf (incWit s1))"
-                  "w \<in> sameLocWrites (incCommitted s1) a"
+                  "w \<in> sameLocWritesSet (incCommitted s1) a"
         | "rf (incWit s2) = rf (incWit s1)"
 proof (cases rule: monStepE_rf[OF monStep])
   case 1
   thus ?thesis
     using that
-    by (cases rule: monAddToRfLoadE[OF 1(2) inv]) auto
+    by (cases rule: monAddToRfLoadE[OF 1(2)]) auto
 next
   case 2
   thus ?thesis
     using that
-    by (cases rule: monAddToRfRmwE[OF 2(2) inv]) auto
+    by (cases rule: monAddToRfRmwE[OF 2(2)]) auto
 next
   case 3
   thus ?thesis using that by auto
@@ -2704,18 +2894,18 @@ lemma monStepE_rf_pair [elim?]:
       and inv:     "monInvariant pre s1"
       and in_rf:   "(x, y) \<in> rf (incWit s2)"
   obtains "y = a"
-          "x \<in> sameLocWrites (incCommitted s1) a"
+          "x \<in> sameLocWritesSet (incCommitted s1) a"
         | "(x, y) \<in> rf (incWit s1)"
-          "x \<in> incCommitted s1"
-          "y \<in> incCommitted s1"
+          "x \<in> incCommittedSet s1"
+          "y \<in> incCommittedSet s1"
 proof -
-  have cons_rf: "well_formed_rf (preRestrict pre (incCommitted s1), incWit s1, [])"
+  have cons_rf: "well_formed_rf (preRestrict pre (incCommittedSet s1), incWit s1, [])"
     using inv by auto
-  hence incCom_s1: "(x, y) \<in> rf (incWit s1) \<Longrightarrow> x \<in> incCommitted s1 \<and> y \<in> incCommitted s1"
+  hence incCom_s1: "(x, y) \<in> rf (incWit s1) \<Longrightarrow> x \<in> incCommittedSet s1 \<and> y \<in> incCommittedSet s1"
     by auto
   show ?thesis
     using incCom_s1 in_rf that
-    by (cases rule: monStepE_rf2[OF monStep inv]) auto
+    by (cases rule: monStepE_rf2[OF monStep]) auto
 qed
 
 subsubsection {* mo *}
@@ -2761,7 +2951,7 @@ lemma monStepE_mo2 [elim?]:
   obtains (store) "is_write a" 
                   "is_at_atomic_location (lk pre) a"
                   "mo (incWit s2) =    mo (incWit s1)
-                                    \<union> (\<lambda>b. (b, a)) ` sameLocWrites (incCommitted s1) a"
+                                    \<union> (\<lambda>b. (b, a)) ` sameLocWritesSet (incCommitted s1) a"
         | (other) "\<not>is_RMW a"
                   "\<not>(is_store a \<and> is_at_atomic_location (lk pre) a)" 
                   "mo (incWit s2) = mo (incWit s1)"
@@ -2777,18 +2967,18 @@ qed
 lemma monStepE_mo3 [elim?]:
   assumes monStep: "(a, s2) [\<in>] monStep pre s1"
       and inv:     "monInvariant pre s1"
-  obtains "mo (incWit s1) = relRestrict (mo (incWit s2)) (incCommitted s1)"
+  obtains "mo (incWit s1) = relRestrict (mo (incWit s2)) (incCommittedSet s1)"
 proof -
-  have cons_mo: "consistent_mo (preRestrict pre (incCommitted s1), incWit s1, [])"
+  have cons_mo: "consistent_mo (preRestrict pre (incCommittedSet s1), incWit s1, [])"
     using inv by auto
-  hence s1: "mo (incWit s1) = relRestrict (mo (incWit s1)) (incCommitted s1)"
+  hence s1: "mo (incWit s1) = relRestrict (mo (incWit s1)) (incCommittedSet s1)"
     unfolding relRestrict_def by auto 
   show ?thesis
     proof (cases rule: monStepE_mo2[OF monStep inv])
       case 1
-      have "a \<notin> incCommitted s1" using monStep inv by auto
-      hence "  relRestrict (mo (incWit s2)) (incCommitted s1)
-             = relRestrict (mo (incWit s1)) (incCommitted s1)"
+      have "a \<notin> incCommittedSet s1" using monStep inv by auto
+      hence "  relRestrict (mo (incWit s2)) (incCommittedSet s1)
+             = relRestrict (mo (incWit s1)) (incCommittedSet s1)"
         using 1 by auto
       thus ?thesis using 1 s1 that by auto
     next
@@ -2802,10 +2992,10 @@ lemma monStepE_mo_pair [elim?]:
       and inv:     "monInvariant pre s1"
       and in_mo:   "(x, y) \<in> mo (incWit s2)"
   obtains "x \<in> actions0 pre" 
-          "x \<in> incCommitted s1"
+          "x \<in> incCommittedSet s1"
           "y \<in> actions0 pre"
-          "y \<in> incCommitted s2"
-          "y \<notin> incCommitted s1"
+          "y \<in> incCommittedSet s2"
+          "y \<notin> incCommittedSet s1"
           "y = a"
           "x \<noteq> a"
           "loc_of x = loc_of y"
@@ -2815,9 +3005,9 @@ lemma monStepE_mo_pair [elim?]:
           "is_at_atomic_location (lk pre) y"
         | "(x, y) \<in> mo (incWit s1)"
           "x \<in> actions0 pre" 
-          "x \<in> incCommitted s1"
+          "x \<in> incCommittedSet s1"
           "y \<in> actions0 pre"
-          "y \<in> incCommitted s1"
+          "y \<in> incCommittedSet s1"
           "x \<noteq> y"
           "loc_of x = loc_of y"
           "is_write x"
@@ -2825,7 +3015,7 @@ lemma monStepE_mo_pair [elim?]:
           "is_at_atomic_location (lk pre) x"
           "is_at_atomic_location (lk pre) y"
 proof -
-  have cons_mo: "consistent_mo (preRestrict pre (incCommitted s1), incWit s1, [])"
+  have cons_mo: "consistent_mo (preRestrict pre (incCommittedSet s1), incWit s1, [])"
     using inv by auto
   show ?thesis
     proof (cases "(x, y) \<in> mo (incWit s1)")
@@ -2838,21 +3028,21 @@ proof -
       hence "mo (incWit s2) \<noteq> mo (incWit s1)"
         using in_mo by auto
       hence a:     "is_write a" "is_at_atomic_location (lk pre) a"
-        and mo_s2: "mo (incWit s2) = mo (incWit s1) \<union> (\<lambda>b. (b, a)) ` sameLocWrites (incCommitted s1) a"           
+        and mo_s2: "mo (incWit s2) = mo (incWit s1) \<union> (\<lambda>b. (b, a)) ` sameLocWritesSet (incCommitted s1) a"           
         by (auto intro: monStepE_mo2[OF monStep inv])
-      hence x: "x \<in> sameLocWrites (incCommitted s1) a" 
+      hence x: "x \<in> sameLocWritesSet (incCommitted s1) a" 
         and y: "y = a"
         using False in_mo by auto
       hence x2: "is_write x" 
-                "x \<in> incCommitted s1" 
+                "x \<in> incCommittedSet s1" 
                 "loc_of x = loc_of y" 
                 "x \<in> actions0 pre"
         using inv by auto
       hence x3: "is_at_atomic_location (lk pre) x"
         using a y same_loc_atomic_location by metis
-      have a2: "a \<in> incCommitted s2" 
+      have a2: "a \<in> incCommittedSet s2" 
                "a \<in> actions0 pre" 
-               "a \<notin> incCommitted s1"
+               "a \<notin> incCommittedSet s1"
         using monStep inv by auto
       show ?thesis
         using a a2 x x2 x3 y that
@@ -2872,6 +3062,189 @@ lemma monStepE_lo [elim?]:
 using assms
 unfolding monStep_def monPerformActions_def Let_def
 by (cases a) auto
+
+lemma monStepE_lo2 [elim?]:
+  assumes monStep: "(a, s2) [\<in>] monStep pre s1"
+  obtains (lock1) y 
+    where "is_lock a \<or> is_unlock a" 
+          "y \<in> sameLocLocksUnlocksSet (incCommitted s1) a"
+          "lo (incWit s2) = insert (y, a) 
+                                   (   lo (incWit s1) 
+                                     \<union> (\<lambda>c. (c, a)) ` {c \<in> sameLocLocksUnlocksSet (incCommitted s1) a. (c, y) \<in> lo (incWit s1)}
+                                     \<union> Pair a ` {c \<in> sameLocLocksUnlocksSet (incCommitted s1) a. (y, c) \<in> lo (incWit s1)}
+                                   )"
+        | (lock2) "is_lock a \<or> is_unlock a" 
+                  "lo (incWit s2) = lo (incWit s1) \<union> Pair a ` (sameLocLocksUnlocksSet (incCommitted s1) a)"
+        | (other) "\<not>is_lock a" 
+                  "\<not>is_unlock a" 
+                  "lo (incWit s2) = lo (incWit s1)"
+proof (cases rule: monStepE_lo[OF monStep])
+  case 1
+  show ?thesis
+    using that 1(1)
+    by (cases rule: monAddToLoE[OF 1(2)]) auto
+next
+  case 2
+  thus ?thesis using that by auto
+qed
+
+lemma monStepE_lo3 [elim?]:
+  assumes monStep: "(a, s2) [\<in>] monStep pre s1"
+      and inv:     "monInvariant pre s1"
+  obtains "lo (incWit s1) = relRestrict (lo (incWit s2)) (incCommittedSet s1)"
+proof -
+  have cons_lo: "locks_only_consistent_lo (preRestrict pre (incCommittedSet s1), 
+                                           incWit s1, 
+                                           [(''hb'', getHb (preRestrict pre (incCommittedSet s1)) (incWit s1))])"
+    using inv by auto
+  hence s1: "lo (incWit s1) = relRestrict (lo (incWit s1)) (incCommittedSet s1)" by auto
+  show ?thesis
+    proof (cases rule: monStepE_lo2[OF monStep])
+      case 1
+      have "a \<notin> incCommittedSet s1" using monStep inv by auto
+      hence "  relRestrict (lo (incWit s2)) (incCommittedSet s1)
+             = relRestrict (lo (incWit s1)) (incCommittedSet s1)"
+        using 1 by auto
+      thus ?thesis using 1 s1 that by auto
+    next
+      case 2
+      have "a \<notin> incCommittedSet s1" using monStep inv by auto
+      hence "  relRestrict (lo (incWit s2)) (incCommittedSet s1)
+             = relRestrict (lo (incWit s1)) (incCommittedSet s1)"
+        unfolding 2(2) by auto
+      thus ?thesis using 2 s1 that by auto
+    next
+      case 3
+      thus ?thesis using s1 that by auto
+    qed
+qed
+
+lemma monStepE_lo_pair [elim?]:
+  assumes monStep: "(a, s2) [\<in>] monStep pre s1"
+      and inv:     "monInvariant pre s1"
+      and in_lo:   "(x, y) \<in> lo (incWit s2)"
+  obtains "(x, y) \<notin> lo (incWit s1)"
+          "x \<in> actions0 pre" 
+          "x \<in> incCommittedSet s2"
+          "x \<notin> incCommittedSet s1"
+          "y \<in> actions0 pre"
+          "y \<in> incCommittedSet s1"
+          "x = a"
+          "y \<noteq> a"
+          "loc_of x = loc_of y"
+          "is_lock x \<or> is_unlock x"
+          "is_lock y \<or> is_unlock y"
+          "is_at_mutex_location (lk pre) x"
+          "is_at_mutex_location (lk pre) y"
+        | "(x, y) \<notin> lo (incWit s1)"
+          "x \<in> actions0 pre" 
+          "x \<in> incCommittedSet s1"
+          "y \<in> actions0 pre"
+          "y \<in> incCommittedSet s2"
+          "y \<notin> incCommittedSet s1"
+          "y = a"
+          "x \<noteq> a"
+          "loc_of x = loc_of y"
+          "is_lock x \<or> is_unlock x"
+          "is_lock y \<or> is_unlock y"
+          "is_at_mutex_location (lk pre) x"
+          "is_at_mutex_location (lk pre) y"
+        | "(x, y) \<in> lo (incWit s1)"
+          "x \<in> actions0 pre" 
+          "x \<in> incCommittedSet s1"
+          "y \<in> actions0 pre"
+          "y \<in> incCommittedSet s1"
+          "x \<noteq> y"
+          "x \<noteq> a"
+          "y \<noteq> a"
+          "loc_of x = loc_of y"
+          "is_lock x \<or> is_unlock x"
+          "is_lock y \<or> is_unlock y"
+          "is_at_mutex_location (lk pre) x"
+          "is_at_mutex_location (lk pre) y"
+proof -
+
+  have cons_lo: "locks_only_consistent_lo (preRestrict pre (incCommittedSet s1), 
+                                           incWit s1, 
+                                           [(''hb'', getHb (preRestrict pre (incCommittedSet s1)) (incWit s1))])"
+    using inv by auto
+  have loc_kinds: "actions_respect_location_kinds (actions0 pre) (lk pre)"
+    using inv by auto
+  have a2: "a \<in> incCommittedSet s2" 
+           "a \<in> actions0 pre" 
+           "a \<notin> incCommittedSet s1"
+    using monStep inv by auto
+  show ?thesis
+    proof (cases "(x, y) \<in> lo (incWit s1)")
+      case True
+      hence "x \<in> incCommittedSet s1" "y \<in> incCommittedSet s1" using cons_lo by auto
+      hence "x \<noteq> a" "y \<noteq> a" using monStep inv by auto
+      thus ?thesis 
+        using True cons_lo that(3) by auto
+    next
+      case False
+      hence "lo (incWit s2) \<noteq> lo (incWit s1)"
+        using in_lo by auto
+      thus ?thesis
+        proof (cases rule: monStepE_lo2[OF monStep])
+          case (1 z)
+          hence z: "z \<in> actions0 pre" using inv by auto
+          hence loc_z: "is_at_mutex_location (lk pre) z" 
+            using loc_kinds 1(2)
+            unfolding actions_respect_location_kinds_def is_at_mutex_location_def
+            by (cases z) auto
+          hence loc_a: "is_at_mutex_location (lk pre) a"
+            using 1(2) unfolding is_at_mutex_location_def by auto
+          show ?thesis 
+            using 1(3) in_lo False 
+            proof auto
+              assume "y = a" "x = z"
+              have "y \<notin> incCommittedSet s1" using `y = a` monStep inv by auto
+              hence "(x, y) \<notin> lo (incWit s1)" using cons_lo by auto
+              thus ?thesis 
+                using a2 1(1) 1(2) z loc_z loc_a that(2) `y = a` `x = z`
+                unfolding sameLocLocksUnlocksSet_def
+                by auto
+            next
+              assume xy: "y = a" "x \<in> sameLocLocksUnlocksSet (incCommitted s1) a"
+              hence x2: "x \<in> actions0 pre" "is_at_mutex_location (lk pre) x" 
+                using inv loc_a unfolding is_at_mutex_location_def by auto
+              have "y \<notin> incCommittedSet s1" using `y = a` monStep inv by auto
+              hence "(x, y) \<notin> lo (incWit s1)" using cons_lo by auto
+              thus ?thesis 
+                using xy x2 a2 1(1) loc_a that(2)
+                unfolding sameLocLocksUnlocksSet_def
+                by auto
+            next
+              assume xy: "x = a" "y \<in> sameLocLocksUnlocksSet (incCommitted s1) a"
+              hence y2: "y \<in> actions0 pre" "is_at_mutex_location (lk pre) y" 
+                using inv loc_a unfolding is_at_mutex_location_def by auto
+              have "x \<notin> incCommittedSet s1" using `x = a` monStep inv by auto
+              hence "(x, y) \<notin> lo (incWit s1)" using cons_lo by auto
+              thus ?thesis 
+                using xy y2 a2 1(1) loc_a that(1)
+                unfolding sameLocLocksUnlocksSet_def
+                by auto
+            qed
+        next
+          case 2
+          hence xy: "x = a" "y \<in> sameLocLocksUnlocksSet (incCommitted s1) a"
+            using False in_lo by auto
+          hence loc_a: "is_at_mutex_location (lk pre) a"
+            using a2 2(1) loc_kinds
+            unfolding actions_respect_location_kinds_def is_at_mutex_location_def
+            by (cases a) auto
+          hence y2: "y \<in> actions0 pre" "is_at_mutex_location (lk pre) y" 
+            using xy inv unfolding is_at_mutex_location_def by auto
+          have "x \<notin> incCommittedSet s1" using `x = a` monStep inv by auto
+          hence "(x, y) \<notin> lo (incWit s1)" using cons_lo by auto
+          thus ?thesis 
+            using xy y2 a2 2(1) loc_a that(1)
+            unfolding sameLocLocksUnlocksSet_def
+            by auto
+        qed simp
+    qed
+qed
 
 subsubsection {* sc *}
 
@@ -2898,12 +3271,6 @@ by (cases a) auto
 
 subsection {* Simps of checkXxx predicates *}
 
-lemma monCheckConsistency_simp [simp]:
-  shows "  x [\<in>] monCheckConsistency (pre, wit, getRelations pre wit)
-         = axsimpConsistentAlt pre wit"
-unfolding monCheckConsistency_def
-by simp
-
 lemma monCheckWitRestrict_simp [simp]:
   shows "  x [\<in>] monCheckWitRestrict wit1 committed wit2
          = (incWitRestrict wit1 committed = wit2)"
@@ -2926,17 +3293,18 @@ lemma monStep_assumptions:
   shows   "assumptions (incToEx pre s2)" 
 unfolding incToEx_def Let_def
 proof (intro assumptionsI, simp)
-  have rf: "finite_prefixes (rf (incWit s1)) (actions0 (preRestrict pre (incCommitted s1)))"
+  have rf: "finite_prefixes (rf (incWit s1)) (actions0 (preRestrict pre (incCommittedSet s1)))"
     using inv by blast
-  show "finite_prefixes (rf (incWit s2)) (actions0 pre \<inter> incCommitted s2)"
-    proof (cases rule: monStepE_rf2[OF monStep inv])
+  show "finite_prefixes (rf (incWit s2)) (actions0 pre \<inter> incCommittedSet s2)"
+    proof (cases rule: monStepE_rf2[OF monStep])
+oops (*
       case 1
-      show ?thesis sorry
+      show ?thesis 
     next
       case 2
-      show ?thesis sorry
+      show ?thesis 
     qed
-oops
+oops *)
 
 subsubsection {* tot_empty *}
 
@@ -2962,7 +3330,7 @@ lemma monStep_well_formed_threads_opsem:
 proof -
   have "well_formed_threads_opsem (pre, empty_witness, [])"
     using inv by auto
-  hence "well_formed_threads_opsem (preRestrict pre (incCommitted s2), empty_witness, [])"
+  hence "well_formed_threads_opsem (preRestrict pre (incCommittedSet s2), empty_witness, [])"
     using well_formed_threads_opsem_restriction by auto
   thus ?thesis
     unfolding incToEx_def Let_def
@@ -2977,9 +3345,9 @@ lemma monStep_well_formed_rf_aux:
       and rf:      "rf (incWit s2) = rf (incWit s1)"
   shows   "well_formed_rf (incToEx pre s2)"
 proof -
-  have cons_rf: "well_formed_rf (preRestrict pre (incCommitted s1), incWit s1, [])"
+  have cons_rf: "well_formed_rf (preRestrict pre (incCommittedSet s1), incWit s1, [])"
     using inv unfolding incToEx_def Let_def by auto
-  have com: "incCommitted s2 = insert a (incCommitted s1)"
+  have com: "incCommitted s2 = a#(incCommitted s1)"
     using monStep by auto
   show ?thesis
     unfolding incToEx_def Let_def well_formed_rf.simps 
@@ -3034,18 +3402,18 @@ lemma monStep_well_formed_rf:
       and inv:     "monInvariant pre s1"
   shows   "well_formed_rf (incToEx pre s2)"
 proof -
-  have cons_rf: "well_formed_rf (preRestrict pre (incCommitted s1), incWit s1, [])"
+  have cons_rf: "well_formed_rf (preRestrict pre (incCommittedSet s1), incWit s1, [])"
     using inv unfolding incToEx_def Let_def by auto
-  have com: "incCommitted s2 = insert a (incCommitted s1)"
+  have com: "incCommitted s2 = a#(incCommitted s1)"
     using monStep by auto
-  have a: "a \<in> incCommitted s2" "a \<in> actions0 pre" "a \<notin> incCommitted s1"
+  have a: "a \<in> incCommittedSet s2" "a \<in> actions0 pre" "a \<notin> incCommittedSet s1"
     using monStep inv by auto
   show ?thesis
     proof (cases rule: monStepE_rf[OF monStep])
       case 1 (* load *)
       hence "is_read a" by (intro is_readI) auto
       show ?thesis
-        proof (cases rule: monAddToRfLoadE[OF 1(2) inv])
+        proof (cases rule: monAddToRfLoadE[OF 1(2)])
           case (1 w) 
           hence wit: "rf (incWit s2) = insert (w, a) (rf (incWit s1))"
             by auto
@@ -3065,7 +3433,7 @@ proof -
       case 2 (* rmw *)
       hence "is_read a" by auto
       show ?thesis
-        proof (cases rule: monAddToRfRmwE[OF 2(2) inv])
+        proof (cases rule: monAddToRfRmwE[OF 2(2)])
           case (1 w)
           hence wit: "rf (incWit s2) = insert (w, a) (rf (incWit s1))"
             by auto
@@ -3090,9 +3458,219 @@ proof -
     qed
 qed
 
-subsubsection {* locks_only_consistent_locks *}
-
 subsubsection {* locks_only_consistent_lo *}
+
+lemma monStep_locks_only_consistent_lo:
+  assumes monStep: "(a, s2) [\<in>] monStep pre s1"
+      and inv:     "monInvariant pre s1"
+  shows   "locks_only_consistent_lo (incToEx pre s2)"
+unfolding incToEx_def Let_def getRelations_simp
+proof (intro locks_only_consistent_loI, simp_all)
+  have cons_lo: "locks_only_consistent_lo (preRestrict pre (incCommittedSet s1), 
+                                           incWit s1, 
+                                           [(''hb'', getHb (preRestrict pre (incCommittedSet s1)) (incWit s1))])"
+    using inv by auto
+  hence trans: "trans (lo (incWit s1))" by auto
+  have a: "a \<notin> incCommittedSet s1" "a \<in> actions0 pre"
+    using monStep inv by auto
+  fix x y
+  assume in_lo_s2: "(x, y) \<in> lo (incWit s2)"
+  show "sameLocLocksUnlocks_cond (preRestrict pre (incCommittedSet s2)) x y"
+    unfolding sameLocLocksUnlocks_cond_def
+    using a monStep
+    by (cases rule: monStepE_lo_pair[OF monStep inv in_lo_s2]) auto
+  show "(y, x) \<notin> getHb (preRestrict pre (incCommittedSet s2)) (incWit s2)"
+    sorry
+  fix z
+  assume yz_in_lo_s2: "(y, z) \<in> lo (incWit s2)"
+  have x: "x \<in> insert a (incCommittedSet s1)"
+          "is_lock x \<or> is_unlock x"
+    using monStepE_lo_pair[OF monStep inv in_lo_s2]
+    by auto
+  have y: "y \<in> insert a (incCommittedSet s1)"
+          "is_lock y \<or> is_unlock y"
+          "loc_of x = loc_of y"
+    using monStepE_lo_pair[OF monStep inv in_lo_s2]
+    by auto
+  have z: "z \<in> insert a (incCommittedSet s1)"
+          "is_lock z \<or> is_unlock z"
+          "loc_of y = loc_of z"
+    using monStepE_lo_pair[OF monStep inv yz_in_lo_s2]
+    by auto
+  show "(x, z) \<in> lo (incWit s2)"
+    proof (cases "x = a \<or> y = a \<or> z = a")
+      case False
+      hence "x \<in> incCommittedSet s1"
+            "y \<in> incCommittedSet s1"
+            "z \<in> incCommittedSet s1"
+        using x y z by auto
+      hence "(x, y) \<in> relRestrict (lo (incWit s2)) (incCommittedSet s1)"
+            "(y, z) \<in> relRestrict (lo (incWit s2)) (incCommittedSet s1)"
+        using in_lo_s2 yz_in_lo_s2 
+        by auto
+      hence "(x, y) \<in> lo (incWit s1)"
+            "(y, z) \<in> lo (incWit s1)"
+        using monStepE_lo3[OF monStep inv] by blast+
+      hence "(x, z) \<in> lo (incWit s1)"
+        using x cons_lo
+        unfolding locks_only_consistent_lo.simps trans_def
+        by metis
+      thus ?thesis
+        using monStepE_lo3[OF monStep inv] by fast
+    next
+      case True
+      show ?thesis
+        proof (cases rule: monStepE_lo2[OF monStep])
+          case (1 w)
+          show ?thesis 
+            proof (cases "x = a")
+              assume "x = a"
+              hence y2: "(w, y) \<in> lo (incWit s1)" "y \<noteq> a" 
+                using in_lo_s2 1(2) 1(3) a cons_lo by auto
+              hence "y \<noteq> w" using cons_lo by auto
+              have "z \<noteq> a"
+                proof
+                  assume "z = a"
+                  hence "(y, z) \<notin> lo (incWit s1)"
+                    using monStepE_lo_pair[OF monStep inv yz_in_lo_s2] by auto
+                  hence "(y, w) \<in> lo (incWit s1)"
+                    using yz_in_lo_s2 1(3) `y \<noteq> w` a(1) y2 by auto
+                  hence "(w, w) \<in> lo (incWit s1)"
+                    using transE[OF trans] y2 by auto
+                  thus False using cons_lo by auto
+                qed
+              hence "(y, z) \<in> lo (incWit s1)"
+                using monStepE_lo_pair[OF monStep inv yz_in_lo_s2] `y \<noteq> a` by auto
+              hence wz_in_lo_s1: "(w, z) \<in> lo (incWit s1)"
+                using transE[OF trans] y2 by auto
+              have "z \<in> sameLocLocksUnlocksSet (incCommitted s1) a"
+                unfolding sameLocLocksUnlocksSet_def 
+                using wz_in_lo_s1 cons_lo y(3) z(3) `x = a` 
+                by auto             
+              thus ?thesis using wz_in_lo_s1 `x = a` 1 by auto
+            next 
+              assume "x \<noteq> a"
+              show ?thesis
+                proof (cases "y = a")
+                  assume "y = a"
+                  have "(x, y) \<notin> lo (incWit s1)"
+                    using monStepE_lo_pair[OF monStep inv in_lo_s2] `y = a` by auto
+                  hence x: "(x, w) \<in> lo (incWit s1) \<or> (x = w)"
+                    using 1(3) in_lo_s2 `y = a` `x \<noteq> a` by auto
+                  have "(y, z) \<notin> lo (incWit s1)"
+                    using monStepE_lo_pair[OF monStep inv yz_in_lo_s2] `y = a` by auto
+                  hence "(w, z) \<in> lo (incWit s1)"
+                    using 1(2) 1(3) yz_in_lo_s2 `y = a` a by auto
+                  hence "(x, z) \<in> lo (incWit s1)"
+                    using x transE[OF trans] by auto 
+                  thus ?thesis using 1 by auto
+                next 
+                  assume "y \<noteq> a"
+                  hence "z = a" using `x \<noteq> a` True by auto
+                  have xy_in_lo_s1: "(x, y) \<in> lo (incWit s1)"
+                    using monStepE_lo_pair[OF monStep inv in_lo_s2] 
+                    using `x \<noteq> a` `y \<noteq> a` 
+                    by metis
+                  have "(y, z) \<notin> lo (incWit s1)"
+                    using monStepE_lo_pair[OF monStep inv yz_in_lo_s2] `z = a` by auto
+                  hence "(y, w) \<in> lo (incWit s1) \<or> (y = w)"
+                    using yz_in_lo_s2 `z = a` `y \<noteq> a` 1(3) by auto
+                  hence xw_in_lo_s1: "(x, w) \<in> lo (incWit s1)"
+                    using xy_in_lo_s1 using transE[OF trans] by auto 
+                  have "x \<in> sameLocLocksUnlocksSet (incCommitted s1) a"
+                    unfolding sameLocLocksUnlocksSet_def 
+                    using xy_in_lo_s1 cons_lo y(3) z(3) `z = a` 
+                    by auto
+                  thus ?thesis using xw_in_lo_s1 `z = a` 1 by auto
+                qed
+            qed
+        next
+          case 2
+          have mo1: "lo (incWit s1) = relRestrict (lo (incWit s2)) (incCommittedSet s1)"
+            using monStepE_lo3[OF monStep inv] by auto
+          have "y \<noteq> a" "z \<noteq> a"
+            using in_lo_s2 yz_in_lo_s2 a
+            unfolding 2(2) 
+            using mo1
+            by auto
+          hence "x = a" using True by auto
+          hence "loc_of a = loc_of z"
+            using y z by auto
+          hence "z \<in> sameLocLocksUnlocksSet (incCommitted s1) a"
+            unfolding sameLocLocksUnlocksSet_def
+            using z `z \<noteq> a`
+            by auto
+          thus ?thesis using 2(2) `x = a` by auto
+        next
+          case 3
+          hence False using True x y z by auto
+          thus ?thesis by auto
+        qed
+    qed
+next
+  have cons_lo: "locks_only_consistent_lo (preRestrict pre (incCommittedSet s1), 
+                                           incWit s1, 
+                                           [(''hb'', getHb (preRestrict pre (incCommittedSet s1)) (incWit s1))])"
+    using inv by auto
+  fix x y
+  assume xy: "x \<in> actions0 pre \<and> x \<in> incCommittedSet s2"
+             "y \<in> actions0 pre \<and> y \<in> incCommittedSet s2"
+             "x \<noteq> y"
+             "loc_of x = loc_of y"
+             "is_lock x \<or> is_unlock x"
+             "is_lock y \<or> is_unlock y"
+             "is_at_mutex_location (lk pre) x"
+             "is_at_mutex_location (lk pre) y"
+  show "(x, y) \<in> lo (incWit s2) \<or> (y, x) \<in> lo (incWit s2)"
+    proof (cases "x = a \<or> y = a", simp_all)
+      assume "x = a \<or> y = a"
+      hence monAddToLo: "lo (incWit s2) [\<in>] monAddToLo pre a s1"
+        using monStepE_lo[OF monStep] xy by auto
+      have loc: "is_at_mutex_location (lk pre) a"
+        using `x = a \<or> y = a` xy by auto
+      let ?x2 = "if x = a then x else y"
+      let ?y2 = "if x = a then y else x"
+      have x2: "?x2 = a"                 
+        using `x = a \<or> y = a` by auto
+      hence "?y2 \<in> incCommittedSet s1"
+        using xy monStep by auto
+      hence y2: "?y2 \<in> sameLocLocksUnlocksSet (incCommitted s1) a"
+        using x2 xy unfolding sameLocLocksUnlocksSet_def by (cases "x = a") auto
+      have "(?x2, ?y2) \<in> lo (incWit s2) \<or> (?y2, ?x2) \<in> lo (incWit s2)"
+        using monAddToLo
+        proof (cases rule: monAddToLoE)
+          case (1 z)
+          hence loc_z: "is_at_mutex_location (lk pre) z"
+            unfolding sameLocLocksUnlocksSet_def
+            using same_loc_mutex_location[OF loc, where b=z] 
+            by simp blast
+          have "z \<in> actions0 pre"
+            using 1 inv by auto
+          hence "(?y2, z) \<notin> lo (incWit s1) \<Longrightarrow> ?y2 \<noteq> z \<Longrightarrow> (z, ?y2) \<in> lo (incWit s1)"
+            using 1(1) y2 loc_z xy(1) xy(2)
+            unfolding sameLocLocksUnlocksSet_def
+            by (cases rule: locks_only_consistent_loE2_inv[OF cons_lo]) auto
+          thus ?thesis using 1 x2 y2 by blast
+        next
+          case 2
+          thus ?thesis using x2 y2 by auto
+        qed
+      thus ?thesis by (cases "x = a") auto
+    next
+      assume "x \<noteq> a \<and> y \<noteq> a"
+      hence xy2: "x \<in> incCommittedSet s1" 
+                 "y \<in> incCommittedSet s1"
+        using xy monStep by auto
+      have "(x, y) \<in> lo (incWit s1) \<or> (y, x) \<in> lo (incWit s1)"
+        using cons_lo xy xy2
+        unfolding locks_only_consistent_lo.simps
+        by auto
+      thus ?thesis
+        using monStepE_lo3[OF monStep inv] by fast
+    qed
+qed
+
+subsubsection {* locks_only_consistent_locks *}
 
 subsubsection {* consistent_mo *}
 
@@ -3102,13 +3680,13 @@ lemma monStep_consistent_mo:
   shows   "consistent_mo (incToEx pre s2)"
 unfolding incToEx_def Let_def
 proof (intro consistent_moI, simp_all)
-  have cons_mo: "consistent_mo (preRestrict pre (incCommitted s1), incWit s1, [])"
+  have cons_mo: "consistent_mo (preRestrict pre (incCommittedSet s1), incWit s1, [])"
     using inv by auto
-  have a: "a \<notin> incCommitted s1" "a \<in> actions0 pre"
+  have a: "a \<notin> incCommittedSet s1" "a \<in> actions0 pre"
     using monStep inv by auto
   fix x y
   assume in_mo_s2: "(x, y) \<in> mo (incWit s2)"
-  show "sameLocAtWrites (preRestrict pre (incCommitted s2)) x y"
+  show "sameLocAtWrites (preRestrict pre (incCommittedSet s2)) x y"
     unfolding sameLocAtWrites_def
     using a monStep
     by (cases rule: monStepE_mo_pair[OF monStep inv in_mo_s2]) auto
@@ -3118,21 +3696,21 @@ proof (intro consistent_moI, simp_all)
     using monStepE_mo_pair[OF monStep inv yz_in_mo_s2] by auto
   hence z2: "is_store z \<or> is_RMW z"
     by (cases z) auto
-  have "y \<in> incCommitted s1" "loc_of y = loc_of z"
+  have "y \<in> incCommittedSet s1" "loc_of y = loc_of z"
     using monStepE_mo_pair[OF monStep inv yz_in_mo_s2] by auto
-  hence x: "x \<in> incCommitted s1" 
+  hence x: "x \<in> incCommittedSet s1" 
            "(x, y) \<in> mo (incWit s1)"
            "x \<in> actions0 pre"
            "is_write x"
            "loc_of x = loc_of z"
     using monStepE_mo_pair[OF monStep inv in_mo_s2] by auto
-  hence x2: "x \<in> sameLocWrites (incCommitted s1) z"
+  hence x2: "x \<in> sameLocWritesSet (incCommitted s1) z"
     unfolding sameLocWrites_def by auto
   show "(x, z) \<in> mo (incWit s2)"
     proof (cases "z = a")
       assume "z = a"
       hence "  mo (incWit s2)
-             = mo (incWit s1) \<union> (\<lambda>b. (b, a)) ` sameLocWrites (incCommitted s1) a"
+             = mo (incWit s1) \<union> (\<lambda>b. (b, a)) ` sameLocWritesSet (incCommitted s1) a"
         using z z2 monStepE_mo2[OF monStep inv] by metis
       thus ?thesis using x2 `z = a` by auto
     next
@@ -3147,11 +3725,11 @@ proof (intro consistent_moI, simp_all)
         using monStepE_mo2[OF monStep inv] by fast
     qed
 next
-  have cons_mo: "consistent_mo (preRestrict pre (incCommitted s1), incWit s1, [])"
+  have cons_mo: "consistent_mo (preRestrict pre (incCommittedSet s1), incWit s1, [])"
     using inv by auto
   fix x y
-  assume xy: "x \<in> actions0 pre \<and> x \<in> incCommitted s2"
-             "y \<in> actions0 pre \<and> y \<in> incCommitted s2"
+  assume xy: "x \<in> actions0 pre \<and> x \<in> incCommittedSet s2"
+             "y \<in> actions0 pre \<and> y \<in> incCommittedSet s2"
              "x \<noteq> y"
              "loc_of x = loc_of y"
              "is_write x"
@@ -3166,35 +3744,35 @@ next
     proof (cases "x = a")
       assume "x = a"
       hence mo_s2: "  mo (incWit s2)
-                    = mo (incWit s1) \<union> (\<lambda>b. (b, a)) ` sameLocWrites (incCommitted s1) a"
+                    = mo (incWit s1) \<union> (\<lambda>b. (b, a)) ` sameLocWritesSet (incCommitted s1) a"
         using xy x2 monStepE_mo2[OF monStep inv] by metis
-      have "y \<in> incCommitted s1"
+      have "y \<in> incCommittedSet s1"
         using xy `x = a` monStep by auto
-      hence "y \<in> sameLocWrites (incCommitted s1) x"
+      hence "y \<in> sameLocWritesSet (incCommitted s1) x"
         using xy unfolding sameLocWrites_def by auto
       hence "(y, x) \<in> mo (incWit s2)"
         using `x = a` mo_s2 by auto
       thus ?thesis by auto
     next
       assume "x \<noteq> a"
-      have x3: "x \<in> incCommitted s1"
+      have x3: "x \<in> incCommittedSet s1"
         using xy `x \<noteq> a` monStep by auto
       show ?thesis
         proof (cases "y = a")
           assume "y = a"
           hence mo_s2: "  mo (incWit s2)
-                        = mo (incWit s1) \<union> (\<lambda>b. (b, a)) ` sameLocWrites (incCommitted s1) a"
+                        = mo (incWit s1) \<union> (\<lambda>b. (b, a)) ` sameLocWritesSet (incCommitted s1) a"
             using xy y2 monStepE_mo2[OF monStep inv] by metis
-          have "x \<in> incCommitted s1"
+          have "x \<in> incCommittedSet s1"
             using xy `y = a` monStep by auto
-          hence "x \<in> sameLocWrites (incCommitted s1) y"
+          hence "x \<in> sameLocWritesSet (incCommitted s1) y"
             using xy unfolding sameLocWrites_def by auto
           hence "(x, y) \<in> mo (incWit s2)"
             using `y = a` mo_s2 by auto
           thus ?thesis by auto
         next
           assume "y \<noteq> a"
-          have y3: "y \<in> incCommitted s1"
+          have y3: "y \<in> incCommittedSet s1"
             using xy `y \<noteq> a` monStep by auto
           have "(x, y) \<in> mo (incWit s1) \<or> (y, x) \<in> mo (incWit s1)"
             using cons_mo xy x3 y3
@@ -3228,24 +3806,24 @@ lemma monStep_rmw_atomicity:
   shows   "rmw_atomicity (incToEx pre s2)"
 unfolding incToEx_def Let_def
 proof (intro rmw_atomicityI, clarsimp)
-  have cons_rf: "well_formed_rf (preRestrict pre (incCommitted s1), incWit s1, [])"
+  have cons_rf: "well_formed_rf (preRestrict pre (incCommittedSet s1), incWit s1, [])"
     using inv by auto
-  have cons_mo: "consistent_mo (preRestrict pre (incCommitted s1), incWit s1, [])"
+  have cons_mo: "consistent_mo (preRestrict pre (incCommittedSet s1), incWit s1, [])"
     using inv by auto
-  have cons_rmw: "rmw_atomicity (preRestrict pre (incCommitted s1), incWit s1, [])"
+  have cons_rmw: "rmw_atomicity (preRestrict pre (incCommittedSet s1), incWit s1, [])"
     using inv by auto
-  have com: "incCommitted s2 = insert a (incCommitted s1)"
+  have com: "incCommitted s2 = a#(incCommitted s1)"
     using monStep by auto
   fix w r
-  assume w: "w \<in> actions0 pre" "w \<in> incCommitted s2"
-     and r: "r \<in> actions0 pre" "r \<in> incCommitted s2" "is_RMW r"
-  have a: "a \<notin> incCommitted s1" "a \<in> actions0 pre"
+  assume w: "w \<in> actions0 pre" "w \<in> incCommittedSet s2"
+     and r: "r \<in> actions0 pre" "r \<in> incCommittedSet s2" "is_RMW r"
+  have a: "a \<notin> incCommittedSet s1" "a \<in> actions0 pre"
     using monStep inv by auto
   hence "(a, r) \<notin> rf (incWit s1)"
     using cons_rf by auto
   hence "(a, r) \<notin> rf (incWit s2)"
     using a
-    by (cases rule: monStepE_rf2[OF monStep inv]) auto
+    by (cases rule: monStepE_rf2[OF monStep]) auto
   have "(a, r) \<notin> mo (incWit s1)"
     using a cons_mo by auto
   hence "(a, r) \<notin> mo (incWit s2)"
@@ -3253,77 +3831,77 @@ proof (intro rmw_atomicityI, clarsimp)
     by (cases rule: monStepE_mo2[OF monStep inv]) auto
   have "(w, a) \<notin> rf (incWit s1)"
     using a cons_rf by auto
-  show "adjacent_less_than (mo (incWit s2)) (actions0 pre \<inter> incCommitted s2) w r 
+  show "adjacent_less_than (mo (incWit s2)) (actions0 pre \<inter> incCommittedSet s2) w r 
         = ((w, r) \<in> rf (incWit s2))"
     proof (cases "w = a")
       assume "w = a"
-      have "\<not>adjacent_less_than (mo (incWit s2)) (actions0 pre \<inter> incCommitted s2) a r "
+      have "\<not>adjacent_less_than (mo (incWit s2)) (actions0 pre \<inter> incCommittedSet s2) a r "
         using `(a, r) \<notin> mo (incWit s2)` by auto
       thus ?thesis
         using `(a, r) \<notin> rf (incWit s2)` `w = a` by auto
     next
       assume "w \<noteq> a"
-      hence w2: "w \<in> incCommitted s1"
+      hence w2: "w \<in> incCommittedSet s1"
         using w monStep by auto
       show ?thesis
         proof (cases "r = a")
           assume "r \<noteq> a"
-          hence r2: "r \<in> incCommitted s1"
+          hence r2: "r \<in> incCommittedSet s1"
             using r monStep by auto
           have mo_eq: "((w, r) \<in> mo (incWit s1)) = ((w, r) \<in> mo (incWit s2))"
             using w w2 r r2 by (cases rule: monStepE_mo3[OF monStep inv]) auto       
-          have "  (\<exists>z\<in>actions0 pre \<inter> incCommitted s2. 
+          have "  (\<exists>z\<in>actions0 pre \<inter> incCommittedSet s2. 
                        (w, z) \<in> mo (incWit s2) \<and> (z, r) \<in> mo (incWit s2))
-                 = (\<exists>z\<in>actions0 pre \<inter> incCommitted s1. 
+                 = (\<exists>z\<in>actions0 pre \<inter> incCommittedSet s1. 
                        (w, z) \<in> mo (incWit s1) \<and> (z, r) \<in> mo (incWit s1))"
             unfolding com
             using `(a, r) \<notin> mo (incWit s2)` w2 r2
             by (cases rule: monStepE_mo3[OF monStep inv]) auto
-          hence "  adjacent_less_than (mo (incWit s2)) (actions0 pre \<inter> incCommitted s2) w r
-                = adjacent_less_than (mo (incWit s1)) (actions0 pre \<inter> incCommitted s1) w r"
+          hence "  adjacent_less_than (mo (incWit s2)) (actions0 pre \<inter> incCommittedSet s2) w r
+                = adjacent_less_than (mo (incWit s1)) (actions0 pre \<inter> incCommittedSet s1) w r"
             unfolding adjacent_less_than_def using mo_eq by auto
           also have "... = ((w, r) \<in> rf (incWit s1))"
             using cons_rmw w w2 r r2 by auto
           also have "... = ((w, r) \<in> rf (incWit s2))"
             using `r \<noteq> a`
-            by (cases rule: monStepE_rf2[OF monStep inv]) auto
+            by (cases rule: monStepE_rf2[OF monStep]) auto
           finally show ?thesis .
         next
           assume "r = a"
           hence "is_RMW a" using r by auto
           hence mo_s2: "  mo (incWit s2)
-                        = mo (incWit s1) \<union> (\<lambda>b. (b, a)) ` sameLocWrites (incCommitted s1) a"
+                        = mo (incWit s1) \<union> (\<lambda>b. (b, a)) ` sameLocWritesSet (incCommitted s1) a"
              by (cases rule: monStepE_mo2[OF monStep inv]) auto
           have rmw_step: "rf (incWit s2) [\<in>] monAddToRfRmw pre a s1"
             using `is_RMW a`
             by (cases rule: monStepE_rf[OF monStep], cases a) auto
           show ?thesis
-            proof (cases "w \<in> sameLocWrites (incCommitted s1) a")
-              assume w_not_same_loc: "w \<notin> sameLocWrites (incCommitted s1) a"
+            proof (cases "w \<in> sameLocWritesSet (incCommitted s1) a")
+              assume w_not_same_loc: "w \<notin> sameLocWritesSet (incCommitted s1) a"
               hence "(w, a) \<notin> rf (incWit s2)"
                 using `(w, a) \<notin> rf (incWit s1)` 
-                by (cases rule: monAddToRfRmwE[OF rmw_step inv]) auto
+                by (cases rule: monAddToRfRmwE[OF rmw_step]) auto
               have "(w, a) \<notin> mo (incWit s1)"
                 using a cons_mo by auto
               hence "(w, a) \<notin> mo (incWit s2)"
                  using w_not_same_loc mo_s2 by auto
-              hence "\<not> adjacent_less_than (mo (incWit s2)) (actions0 pre \<inter> incCommitted s2) w a"
+              hence "\<not> adjacent_less_than (mo (incWit s2)) (actions0 pre \<inter> incCommittedSet s2) w a"
                  by auto                 
               thus ?thesis 
                 using `r = a` `(w, a) \<notin> rf (incWit s2)` by auto
             next
-              assume w_same_loc: "w \<in> sameLocWrites (incCommitted s1) a"
-              then obtain w' where w':     "w' \<in> sameLocWrites (incCommitted s1) a"
-                               and w'_max: "\<forall>w''\<in>sameLocWrites (incCommitted s1) a. 
+              assume w_same_loc: "w \<in> sameLocWritesSet (incCommitted s1) a"
+              then obtain w' where w':     "w' \<in> sameLocWritesSet(incCommitted s1) a"
+                               and w'_max: "\<forall>w''\<in>sameLocWritesSet (incCommitted s1) a. 
                                                   (w', w'') \<notin> mo (incWit s1)"
                                and rf_s2:  "rf (incWit s2) = insert (w', a) (rf (incWit s1))"
-                by (cases rule: monAddToRfRmwE[OF rmw_step inv]) auto
+                by (cases rule: monAddToRfRmwE[OF rmw_step]) auto
               have w'_a_in_mo: "(w', a) \<in> mo (incWit s2)"
                 using w' mo_s2 by auto
               show ?thesis
                 proof (cases "w = w'")
                   assume "w = w'"
-                  have "adjacent_less_than (mo (incWit s2)) (actions0 pre \<inter> incCommitted s2) w' a"
+                  have "adjacent_less_than (mo (incWit s2)) (actions0 pre \<inter> incCommittedSet s2) w' a"
                     unfolding adjacent_less_than_def
                     using w'_a_in_mo
                     proof auto
@@ -3331,7 +3909,7 @@ proof (intro rmw_atomicityI, clarsimp)
                       assume "(z, a) \<in> mo (incWit s2)"
                       moreover have "(z, a) \<notin> mo (incWit s1)"
                         using a cons_mo by auto
-                      ultimately have "z \<in> sameLocWrites (incCommitted s1) a"
+                      ultimately have "z \<in> sameLocWritesSet (incCommitted s1) a"
                         using mo_s2 by auto
                       hence "(w', z) \<notin> mo (incWit s1)" "z \<noteq> a"
                         using w'_max a by auto
@@ -3346,12 +3924,12 @@ proof (intro rmw_atomicityI, clarsimp)
                   hence "(w, a) \<notin> rf (incWit s2)"
                     using rf_s2 `(w, a) \<notin> rf (incWit s1)` by auto
                   have w'2: "w' \<in> actions0 pre" 
-                            "w' \<in> incCommitted s1"
+                            "w' \<in> incCommittedSet s1"
                             "is_write w'"
                             "loc_of w' = loc_of a"
                     using w' inv by auto
                   have w2: "w \<in> actions0 pre" 
-                           "w \<in> incCommitted s1"
+                           "w \<in> incCommittedSet s1"
                            "is_write w"
                            "loc_of w = loc_of a"
                     using w_same_loc inv by auto
@@ -3369,7 +3947,7 @@ proof (intro rmw_atomicityI, clarsimp)
                     using w'_max w_same_loc by auto
                   hence "(w, w') \<in> mo (incWit s2)" 
                     using mo_s2 by auto
-                  hence "\<not> adjacent_less_than (mo (incWit s2)) (actions0 pre \<inter> incCommitted s2) w a"
+                  hence "\<not> adjacent_less_than (mo (incWit s2)) (actions0 pre \<inter> incCommittedSet s2) w a"
                      unfolding adjacent_less_than_def
                      using w'_a_in_mo w'2 com
                      by auto
@@ -3389,14 +3967,47 @@ lemma monStepInvariant:
       and inv:     "monInvariant pre s1"
   shows   "monInvariant pre s2"
 proof -
-  have "finite (actions0 pre)"
+  have finite: "finite (actions0 pre)"
     using inv by auto
+  have committed: "incCommittedSet s2 \<subseteq> actions0 pre"
+    using monStep finite inv
+    unfolding monStep_def Let_def monInvariant_def 
+    by auto
+  have cons: "() [\<in>] monCheckConsistency (incToEx pre s2)"
+    using monStep  
+    unfolding monStep_def Let_def incToEx_def
+    by auto
+  hence "axsimpConsistentAlt (preRestrict pre (incCommittedSet s2)) (incWit s2)"
+    using monStep_tot_empty[OF monStep inv]
+    using monStep_well_formed_threads_opsem[OF monStep inv]
+    using monStep_well_formed_rf[OF monStep inv]
+    using monStep_consistent_mo[OF monStep inv]
+    using monStep_rmw_atomicity[OF monStep inv]
+    unfolding incToEx_def Let_def monCheckConsistency_def
+    by (intro axsimpConsistentI) auto
   thus ?thesis
-    using monStep inv
+    using inv committed
     unfolding monInvariant_def
-    unfolding monStep_def Let_def
-    apply auto sorry (* Not true yet *)
+    by auto
 qed
+
+lemma monTraceInvariant:
+  assumes monTrace: "monTrace pre s1 s2"
+      and init:     "s1 = incInitialState pre"
+  shows   "monInvariant pre s2"
+using assms
+proof induct
+  case (monReflexive pre s)
+  thus "monInvariant pre s"
+    unfolding monInvariant_def
+    by auto
+next
+  case (monStep pre x y z a)
+  thus "monInvariant pre z"
+    using monStepInvariant by auto
+qed
+
+subsubsection {* Soundness *}
 
 lemma monStepSoundness:
   assumes monStep: "(a, s2) [\<in>] monStep pre s1"
@@ -3405,18 +4016,43 @@ lemma monStepSoundness:
 using monStep inv
 using monStepInvariant[OF monStep inv]
 unfolding monInvariant_def
-          monStep_def Let_def incStep_def
+          monStep_def Let_def incStep_def incToEx_def
 by auto
+
+lemma monTraceSoundness_aux:
+  assumes monTrace: "monTrace pre s1 s2"
+      and init:     "s1 = incInitialState pre"
+  shows   "incTrace pre s1 s2"
+using assms
+proof induct
+  case (monReflexive pre s)
+  thus "incTrace pre s s"
+    using incReflexive by auto
+next
+  case (monStep pre x y z a)
+  hence "incStep pre y z a" 
+    using monStepSoundness monTraceInvariant
+    by auto
+  thus "incTrace pre x z"
+    using monStep incStep by auto
+qed
+
+corollary monTraceSoundness:
+  assumes "monTrace pre (incInitialState pre) s"
+  shows   "incTrace pre (incInitialState pre) s"
+using assms monTraceSoundness_aux by simp
 
 subsection {* Completeness *}
 
-(* modification order *)
+subsubsection {* modification order *}
 
 lemma step_mo_not_atomic_write:
   assumes cons:      "axsimpConsistentAlt pre' wit'"
+      and wit:       "(incWit s) = incWitRestrict wit' committed"
       and committed: "actions0 pre' = insert a committed"
       and a:         "is_at_non_atomic_location (lk pre') a \<or> \<not> is_write a"
-  shows              "mo wit' = mo (incWitRestrict wit' committed)"
+  shows              "mo wit' = mo (incWit s)"
+unfolding wit
 proof auto
   fix b c
   assume in_mo: "(b, c) \<in> mo wit'"
@@ -3428,78 +4064,1137 @@ proof auto
     using b c committed by auto
 qed
 
-(*
 lemma step_mo_atomic_write:
-  assumes cons1:     "axsimpConsistentAlt pre  wit"
-      and cons2:     "axsimpConsistentAlt pre' wit'"
-      and wit:       "wit = incWitRestrict wit' (actions0 pre)"
-      and committed: "actions0 pre' = insert a (actions0 pre)"
-      and a:         "  is_at_atomic_location (lk pre') a \<and> is_write a 
-                      \<and> a \<in> actions0 pre \<and> a \<notin> incCommitted s"
+  assumes cons2:      "axsimpConsistentAlt pre' wit'"
+      and wit:        "(incWit s) = incWitRestrict wit' (incCommittedSet s)"
+      and committed:  "actions0 pre' = insert a (incCommittedSet s)"
+      and downclosed: "downclosed (incCommittedSet s) (mo wit')"
+      and a:          "is_at_atomic_location (lk pre') a"
+                      "is_write a"
+                      "a \<in> actions0 pre'"
+                      "a \<notin> incCommittedSet s"
   shows   "mo wit' [\<in>] monAddToMo pre a s"
 unfolding monAddToMo_def Let_def
 proof simp
-  let ?succ     = "(\<lambda>b. (b, a)) ` {x \<in> actions0 pre. x \<in> incCommitted s \<and> x \<noteq> a \<and> is_write x \<and> loc_of x = loc_of a}"
+  let ?succ     = "(\<lambda>b. (b, a)) ` sameLocWritesSet (incCommitted s) a"
   let ?new_mo   = "mo (incWit s) \<union> ?succ"
-  show "mo (incWit s')  = ?new_mo"
+  show "mo wit' = ?new_mo"
     proof (intro equalityI subsetI)
       fix x
-      assume "x \<in> mo (incWit s')"
-      then obtain b c where "(b, c) = x" "(b, c) \<in> mo (incWit s')" by (cases x) fast
+      assume "x \<in> mo wit'"
+      then obtain b c where x:     "(b, c) = x" 
+                        and in_mo: "(b, c) \<in> mo wit'" by (cases x) fast
       have "(b, c) \<in> ?new_mo"
-        proof (cases "b = a")
+        proof (cases "c = a")
         next
-          assume "b = a"
-          have not_in_mo_bc: "(b, c) \<notin> mo (incWit s)" using a wit `b = a` by auto
-          have "(c, b) \<notin> mo (incWit s')" 
-            using consistent_mo_aux2[OF cons2 `(b, c) \<in> mo (incWit s')`] by simp
-          hence not_in_mo_cb: "(c, b) \<notin> mo (incWit s)" using wit by auto 
-          have "c \<notin> incCommitted s"
-            proof
-              assume "c \<in> incCommitted s"
-              have "b \<in> actions0 pre \<and> c \<in> actions0 pre \<and> b \<noteq> c \<and> 
-                    is_write b \<and> is_write c \<and> loc_of b = loc_of c \<and> 
-                    is_at_atomic_location (lk pre) b"
-                using consistent_mo_aux2[OF cons2 `(b, c) \<in> mo (incWit s')`] incCommitted
-                by auto
-              hence "(b, c) \<in> mo (incWit s) \<or> (c, b) \<in> mo (incWit s)"
-                using `c \<in> incCommitted s` consistent_mo_aux1[OF cons1] by auto
-              thus False using not_in_mo_bc not_in_mo_cb by simp
-              qed
-          hence "(b, c) \<in> ?succ"
-            using `b = a` consistent_mo_aux2[OF cons2 `(b, c) \<in> mo (incWit s')`] by auto
-          thus "(b, c) \<in> ?new_mo" by simp
+          assume "c = a"
+          hence b: "is_write b" 
+                   "loc_of b = loc_of a" 
+                   "b \<in> actions0 pre'" 
+                   "b \<noteq> a"
+            using in_mo cons2 by auto
+          hence "b \<in> incCommittedSet s" using committed by auto
+          hence "b \<in> sameLocWritesSet (incCommitted s) a"
+            unfolding sameLocWrites_def using b by auto
+          thus "(b, c) \<in> ?new_mo" using `c = a` by simp
         next
-          assume "b \<noteq> a"
-          hence "b \<in> incCommitted s" 
-            using consistent_mo_aux2[OF cons2 `(b, c) \<in> mo (incWit s')`] incCommitted by auto  
-          hence "(b, c) \<in> mo (incWit s)"
-            using wit `(b, c) \<in> mo (incWit s')` by auto
+          assume "c \<noteq> a"
+          have "c \<in> actions0 pre'" using in_mo cons2 by auto
+          hence c: "c \<in> incCommittedSet s" using committed `c \<noteq> a` by simp
+          hence "b \<in> incCommittedSet s" 
+            using downclosed in_mo by (auto elim: downclosedE)
+          hence "(b, c) \<in> mo (incWit s)" using wit in_mo c by auto
           thus "(b, c) \<in> ?new_mo" by simp
         qed
-      thus "x \<in> ?new_mo" using `(b, c) = x` by simp
+      thus "x \<in> ?new_mo" using x by simp
     next
       fix x
       assume "x \<in> ?new_mo"
-      show "x \<in> mo (incWit s')"
-        using `x \<in> ?new_mo`
+      then obtain b c where x:     "(b, c) = x" 
+                        and in_mo: "(b, c) \<in> ?new_mo" by (cases x) fast
+      have "(b, c) \<in> mo wit'"
+        using in_mo
         proof (elim UnE)
-          assume "x \<in> mo (incWit s)" 
-          thus "x \<in> mo (incWit s')" using wit by auto
+          assume "(b, c) \<in> mo (incWit s)" 
+          thus "(b, c) \<in> mo wit'" using wit by auto
         next
-          assume "x \<in> ?succ"
-          then obtain b c where "(b, c) = x" "(b, c) \<in> ?succ" by (cases x) fast
-          hence "(c, b) \<notin> mo (incWit s')" using consistent_mo_aux2[OF cons2] incCommitted by fast
-          hence "(b, c) \<in> mo (incWit s')"
-            using `(b, c) \<in> ?succ` a cons2 incCommitted 
-            using consistent_mo_aux1[where a=a and b=c and wit="incWit s'"] 
+          assume "(b, c)  \<in> ?succ"
+          thus ?thesis
+            using sameLocInMo[OF _ cons2 committed downclosed a]
             by auto
-          thus "x \<in> mo (incWit s')" using `(b, c) = x` by simp
         qed
+      thus "x \<in> mo wit'" using x by simp
     qed
 qed
-*)
+
+subsubsection {* reads-from *}
+
+lemma step_rf_aux:
+  assumes cons2:      "axsimpConsistentAlt pre' wit'"
+      and downclosed: "downclosed committed (rf wit')"
+      and wit:        "wit = incWitRestrict wit' committed"
+      and committed:  "actions0 pre' = insert a committed"
+      and in_rf:      "(b, c) \<in> rf wit'"
+  shows               "(b, c) \<in> rf wit \<or> (c = a)"
+proof (intro disjCI)
+  assume "c \<noteq> a"
+  have "b \<in> actions0 pre'" "c \<in> actions0 pre'"
+    using in_rf cons2 by auto
+  hence b: "b \<in> insert a committed" 
+    and c: "c \<in> committed"
+    using `c \<noteq> a` committed by auto
+  hence "b \<in> committed" 
+    using in_rf downclosed
+    unfolding downclosed_def 
+    by auto
+  hence "(b, c) \<in> rf (incWitRestrict wit' committed)" 
+    using in_rf c by simp
+  thus "(b, c) \<in> rf wit" using wit by simp
+qed  
+
+lemma step_rf_aux2:
+  assumes cons2:      "axsimpConsistentAlt pre' wit'"
+      and downclosed: "downclosed committed (rf wit')"
+      and wit:        "wit = incWitRestrict wit' committed"
+      and committed:  "actions0 pre' = insert a committed"
+  obtains         "rf wit' = rf wit"
+        | w where "rf wit' = insert (w, a) (rf wit)"
+proof (cases "rf wit' = rf wit")
+  case True
+  thus ?thesis using that by auto
+next
+  case False
+  have "rf wit \<subseteq> rf wit'"
+    using wit by auto
+  then obtain x y where in_rf:  "(x, y) \<in> rf wit'" 
+                    and nin_rf: "(x, y) \<notin> rf wit"
+    using False by auto
+  hence "(x, a) \<in> rf wit'" 
+    using step_rf_aux[OF cons2 downclosed wit committed]
+    by auto
+  hence "rf wit' = insert (x, a) (rf wit)"
+    using `rf wit \<subseteq> rf wit'`
+    proof auto
+      fix u v
+      assume "(u, v) \<in> rf wit'" "(u, v) \<notin> rf wit"
+      thus "v = a"
+        using step_rf_aux[OF cons2 downclosed wit committed] by auto
+      thus "u = x"
+        using `(x, a) \<in> rf wit'` `(u, v) \<in> rf wit'`
+        using cons2
+        by auto
+    qed
+  thus ?thesis using that by auto
+qed
+
+lemma step_rf_non_read:
+  assumes cons2:      "axsimpConsistentAlt pre' wit'"
+      and downclosed: "downclosed committed (rf wit')"
+      and wit:        "wit = incWitRestrict wit' committed"
+      and committed:  "actions0 pre' = insert a committed"
+      and a:          "\<not> is_read a" "a \<notin> committed"
+  shows               "rf wit' = rf wit"
+proof (cases rule: step_rf_aux2[OF cons2 downclosed wit committed])
+  case (2 w)
+  hence "(w, a) \<in> rf wit'" by simp
+  hence "is_read a" using cons2 by auto
+  hence False using a by auto
+  thus ?thesis by simp
+qed 
+
+lemma step_rf_auxAddPairToRf:
+  assumes cons2:      "axsimpConsistentAlt pre' wit'"
+      and downclosed: "downclosed (set committed) (rf wit')"
+      and wit:        "wit = incWitRestrict wit' (set committed)"
+      and committed:  "actions0 pre' = insert a (set committed)"
+      and a:          "a \<notin> (set committed)"
+      and in_rf:      "(w, a) \<in> rf wit'"
+  obtains value0
+          where "w \<in> sameLocWritesSet committed a"
+                "(rf wit', value0, value0) [\<in>] auxAddPairToRf (rf wit) w a"
+proof -
+  have "is_write w" using in_rf cons2 by auto
+  then obtain value_w where value_w: "value_written_by w = Some value_w"
+    by (cases w) auto
+  have "is_read a" using in_rf cons2 by auto
+  then obtain value_a where value_a: "value_read_by a = Some value_a"
+    by (cases a) auto
+  have "value_read_by a = value_written_by w"
+    using in_rf cons2 
+    (* For some reason, auto can't find the proof unless we increase the bounds, or unfold the
+    definition. *)  
+    unfolding axsimpConsistentAlt_def 
+    by auto
+  hence "value_w = value_a"
+    using value_w value_a by auto
+  have "rf wit' = insert (w, a) (rf wit)"
+    using in_rf
+    proof auto
+      fix b c
+      assume "(b, c) \<in> rf wit"
+      thus "(b, c) \<in> rf wit'" using wit by auto
+    next
+      fix b c
+      assume bc_in_rf2:  "(b, c) \<in> rf wit'"
+         and bc_nin_rf1: "(b, c) \<notin> rf wit"
+      have "(b, c) \<in> rf wit \<or> (c = a)"
+        using step_rf_aux[OF cons2 downclosed wit committed bc_in_rf2] .
+      thus "c = a" using bc_nin_rf1 by simp
+      thus "b = w" using bc_in_rf2 cons2 in_rf by auto
+    qed
+  hence inAddPair: "(rf wit', value_w, value_w) [\<in>] auxAddPairToRf (rf wit) w a"
+    using value_w value_a `value_w = value_a`
+    unfolding auxAddPairToRf_def
+    by simp
+  have "w \<in> actions0 pre'" "w \<noteq> a"
+    using in_rf cons2 
+    apply (metis axsimpConsistentE well_formed_rfE)
+    using in_rf cons2 
+    by (metis axsimpConsistentE irreflRf)
+  hence "w \<in> set committed" using committed by auto
+  hence "w \<in> sameLocWritesSet committed a"
+    unfolding sameLocWritesSet_def
+    using in_rf cons2
+    by auto
+  thus thesis
+    using that inAddPair by metis
+qed
+
+lemma step_rf_load:
+  assumes cons2:      "axsimpConsistentAlt pre' wit'"
+      and downclosed: "downclosed (incCommittedSet s) (rf wit')"
+      and wit:        "incWit s = incWitRestrict wit' (incCommittedSet s)"
+      and committed:  "actions0 pre' = insert a (incCommittedSet s)"
+      and a:          "is_load a" "a \<in> actions0 pre'" "a \<notin> incCommittedSet s"
+  shows               "rf wit' [\<in>] monAddToRfLoad pre a s"
+proof (cases rule: step_rf_aux2[OF cons2 downclosed wit committed])
+  case 1
+  thus ?thesis
+    unfolding monAddToRfLoad_def auxAddToRfLoad_def
+    by auto
+next
+  case (2 x)
+  then obtain value0 
+        where "x \<in> sameLocWritesSet (incCommitted s) a"
+              "(rf wit', value0, value0) [\<in>] auxAddPairToRf (rf (incWit s)) x a"
+    using step_rf_auxAddPairToRf[OF cons2 downclosed wit committed a(3)]
+    by auto
+  thus ?thesis
+    unfolding monAddToRfLoad_def auxAddToRfLoad_def
+    by auto
+qed
+
+lemma step_rf_rmw:
+  assumes cons2:         "axsimpConsistentAlt pre' wit'"
+      and downclosed_rf: "downclosed (incCommittedSet s) (rf wit')"
+      and downclosed_mo: "downclosed (incCommittedSet s) (mo wit')"
+      and wit:           "incWit s = incWitRestrict wit' (incCommittedSet s)"
+      and committed:     "actions0 pre' = insert a (incCommittedSet s)"
+      and a:             "is_RMW a" "a \<in> actions0 pre'" "a \<notin> incCommittedSet s"
+  shows                  "rf wit' [\<in>] monAddToRfRmw pre a s"
+proof (cases "sameLocWrites (incCommitted s) a = []")
+  case True
+  hence "\<not> (\<exists>w. (w, a) \<in> rf wit')" 
+    using step_rf_auxAddPairToRf[OF cons2 downclosed_rf wit committed a(3)]
+    by auto
+  hence "rf (incWit s) = rf wit'"
+    using step_rf_aux2[OF cons2 downclosed_rf wit committed] by auto
+  thus ?thesis
+    unfolding monAddToRfRmw_def auxAddToRfRmw_def Let_def
+    using True
+    by auto
+next
+  let ?same_loc_writes = "sameLocWritesSet (incCommitted s) a"
+  let ?S = "{w. w \<in> actions0 pre' \<and> (w, a) \<in> mo wit'}"
+  have "actions_respect_location_kinds (actions0 pre') (lk pre')"
+    using cons2 by auto
+  hence a2: "is_at_atomic_location (lk pre') a" "is_write a"
+    using a(1) is_RMWE_location_kind[OF a(1) a(2)] by auto
+  have eq_sets: "?S = ?same_loc_writes"
+    proof auto
+      fix w'
+      assume w': "w' \<in> sameLocWritesSet (incCommitted s) a"
+      show ca_in_mo: "(w', a) \<in> mo wit'"
+        using sameLocInMo[OF w' cons2 committed downclosed_mo] a a2
+        by auto
+      thus "w' \<in> actions0 pre'" using cons2 by auto
+    next
+      fix w'
+      assume "w' \<in> actions0 pre'" "(w', a) \<in> mo wit'"
+      thus "w' \<in> sameLocWritesSet (incCommitted s) a"
+        unfolding sameLocWritesSet_def
+        using committed cons2
+        by auto
+    qed
+  case False
+  then obtain w' where "w' \<in> ?same_loc_writes" by auto
+  hence non_empty: "?S \<noteq> {}" using eq_sets by auto
+  have "assumptions (pre', wit' , [])" 
+    using cons2 by auto
+  hence "finite_prefixes (mo wit') (actions0 pre')"
+    unfolding assumptions.simps by simp
+  hence finite: "finite ?S"
+    unfolding finite_prefixes_def using a by fast
+  hence "irrefl (mo wit') \<and> trans (mo wit')"
+    using cons2 by auto
+  hence isOrder: "isStrictPartialOrder (mo wit')" unfolding isStrictPartialOrder_def .
+  obtain w where w:   "w \<in> ?S" 
+             and max: "(\<forall>y. y \<in> ?S \<longrightarrow> (w, y) \<notin> mo wit')"
+    using supremum_partial_order[OF finite non_empty isOrder] .
+  have adjacent: "adjacent_less_than (mo wit') (actions0 pre') w a"
+    using w max unfolding adjacent_less_than_def by auto
+  hence in_rf: "(w, a) \<in> rf wit'"
+    using cons2 a by auto
+  then obtain value0 
+        where w:  "w \<in> sameLocWritesSet (incCommitted s) a"
+          and rf: "(rf wit', value0, value0) [\<in>] auxAddPairToRf (rf (incWit s)) w a"
+    using step_rf_auxAddPairToRf[OF cons2 downclosed_rf wit committed a(3)] by auto
+  have max: "\<forall>c\<in>sameLocWritesSet (incCommitted s) a. (w, c) \<notin> mo (incWit s)" 
+    (* TODO: use max to prove this quicker. *)
+    proof 
+      fix c
+      assume sameLoc: "c \<in> sameLocWritesSet (incCommitted s) a"
+      have "actions_respect_location_kinds (actions0 pre') (lk pre')"
+        using cons2 by auto
+      hence "is_at_atomic_location (lk pre') a" "is_write a"
+        using a(1) is_RMWE_location_kind[OF a(1) a(2)] by auto
+      hence ca_in_mo: "(c, a) \<in> mo wit'"
+        using sameLocInMo[OF sameLoc cons2 committed downclosed_mo] a
+        by auto
+      hence "c \<in> actions0 pre'" using cons2 by auto
+      hence "(w, c) \<notin> mo wit'"
+        using adjacent ca_in_mo unfolding adjacent_less_than_def by auto
+      thus "(w, c) \<notin> mo (incWit s)" using wit by auto
+    qed
+  thus ?thesis
+    unfolding monAddToRfRmw_def auxAddToRfRmw_def Let_def
+    using w rf False
+    by auto
+qed
+
+subsubsection {* sc-order*}
+
+lemma step_sc_isnot_sc:
+  assumes cons2:     "axsimpConsistentAlt pre' wit'"
+      and wit:       "incWit s = incWitRestrict wit' (incCommittedSet s)"
+      and committed: "actions0 pre' = insert a (incCommittedSet s)"
+      and n_sc:      "\<not> is_seq_cst a"
+  shows              "sc wit'= sc (incWit s)"
+proof auto
+  fix b c
+  assume "(b, c) \<in> sc (incWit s)"
+  thus "(b, c) \<in> sc wit'" using wit by simp
+next
+  fix b c
+  assume in_sc: "(b, c) \<in> sc wit'"
+  hence "is_seq_cst b" "b \<in> actions0 pre'" 
+        "is_seq_cst c" "c \<in> actions0 pre'"
+     using cons2 by auto
+  hence "b \<in> incCommittedSet s" "c \<in> incCommittedSet s"
+     using cons2 n_sc in_sc committed by auto
+  thus "(b, c) \<in> sc (incWit s)" 
+    using cons2 committed in_sc wit by auto
+qed
+
+lemma step_sc_is_sc:
+  assumes cons2:     "axsimpConsistentAlt pre' wit'"
+      and wit:       "incWit s = incWitRestrict wit' (incCommittedSet s)"
+      and committed: "actions0 pre' = insert a (incCommittedSet s)"
+      and a:         "a \<in> actions0 pre'" "a \<notin> incCommittedSet s"
+      and is_sc:     "is_seq_cst a"
+  shows              "sc wit' [\<in>] monAddToSc pre a s"
+unfolding monAddToSc_def 
+proof -
+  let ?sc_list = "scActions (incCommitted s)"
+  let ?sc_set  = "scActionsSet (incCommitted s)"
+  show "sc wit' [\<in>] addToTransitiveOrder ?sc_list a (sc (incWit s))"
+    proof (cases "\<exists>b. (b, a) \<in> sc wit'")
+      assume max: "\<not> (\<exists>b. (b, a) \<in> sc wit')"
+      have "sc wit' = sc (incWit s) \<union> Pair a ` ?sc_set"
+        proof auto
+          fix c
+          assume "c \<in> scActionsSet (incCommitted s)"
+          hence c: "c \<in> incCommittedSet s" "is_seq_cst c" "c \<in> actions0 pre'"
+            using committed by auto
+          hence "c \<noteq> a" using a by auto
+          have "(c, a) \<notin> sc wit'" using max by auto
+          thus "(a, c) \<in> sc wit'"
+            using cons2 a(1) c is_sc `c \<noteq> a` by auto
+        next
+          fix b c
+          assume "(b, c) \<in> sc (incWit s)"
+          thus "(b, c) \<in> sc wit'" using wit by simp
+        next
+          fix b c
+          assume in_sc: "(b, c) \<in> sc wit'"
+             and not_new: "(b, c) \<notin> Pair a ` scActionsSet (incCommitted s)"
+          have "c \<noteq> a" using in_sc max by auto
+          have c: "is_seq_cst c" "c \<in> actions0 pre'" "b \<in> actions0 pre'"
+            using cons2 in_sc by auto
+          hence "c \<in> incCommittedSet s"
+            using `c \<noteq> a` committed by auto
+          hence "c \<in> scActionsSet (incCommitted s)"
+            unfolding scActionsSet_def
+            using c by auto
+          hence "b \<noteq> a" using not_new by auto
+          hence "b \<in> incCommittedSet s"
+            using committed `b \<in> actions0 pre'` by auto          
+          thus "(b, c) \<in> sc (incWit s)" 
+            using wit in_sc `c \<in> incCommittedSet s` by auto
+        qed
+      thus ?thesis unfolding addToTransitiveOrder_def by auto
+    next
+      assume "\<exists>b'. (b', a) \<in> sc wit'"
+      then obtain b' where b': "(b', a) \<in> sc wit'" by fast
+
+      let ?sc_set2 = "{x. (x, a) \<in> sc wit'}"
+  
+      have "b' \<in> ?sc_set2" using b' by simp
+      hence non_empty: "?sc_set2 \<noteq> {}" by fast
+      have "finite_prefixes (sc wit') (actions0 pre')"
+        using cons2 by auto
+      hence finite: "finite ?sc_set2"
+        unfolding finite_prefixes_def using a by fast
+      have irreflexive: "irrefl (sc wit')"
+      and   transitive:  "trans (sc wit')"
+        using cons2 by auto 
+      hence isOrder: "isStrictPartialOrder (sc wit')" 
+        unfolding isStrictPartialOrder_def by simp
+      obtain b where b:   "b \<in> ?sc_set2" 
+                 and max: "(\<forall>y. y \<in> ?sc_set2 \<longrightarrow> (b, y) \<notin> sc wit')"
+        using supremum_partial_order[OF finite non_empty isOrder] by auto
+      have b2: "b \<in> actions0 pre'" using b cons2 by auto
+      hence b3: "b \<in> incCommittedSet s" "is_seq_cst b" "b \<noteq> a"
+        using b committed cons2 by auto
+
+      let ?prev = "(\<lambda>c. (c, a)) ` {x \<in> incCommittedSet s. is_seq_cst x \<and>
+                                   (x, b) \<in> sc (incWit s)}"
+      let ?succ = "(\<lambda>c. (a, c)) ` {x \<in> incCommittedSet s. is_seq_cst x \<and> 
+                                   (b, x) \<in> sc (incWit s)}"
+
+      have "sc (incWit s) \<subseteq> sc wit'" using wit by auto 
+      moreover have "?prev \<subseteq> sc wit'"
+        proof auto
+          fix c
+          assume "(c, b) \<in> sc (incWit s)"
+          hence "(c, b) \<in> sc wit'" using wit by auto
+          thus "(c, a) \<in> sc wit'" using transitive b transE by auto
+        qed
+      moreover have "?succ \<subseteq> sc wit'"
+        proof auto
+          fix c
+          assume in_sc: "(b, c) \<in> sc (incWit s)"
+          hence c: "c \<in> incCommittedSet s" 
+                   "c \<in> actions0 pre'" 
+                   "is_seq_cst c" 
+            using cons2 wit a by auto
+          have "(b, c) \<in> sc wit'" using in_sc wit by auto
+          hence "(c, a) \<notin> sc wit'" using max c by auto
+          thus "(a, c) \<in> sc wit'" 
+            using cons2 c a is_sc by auto
+        qed
+      moreover have "sc wit' \<subseteq> sc (incWit s) \<union> {(b, a)} \<union> ?prev \<union> ?succ"
+        proof auto
+          fix c d
+          assume in_sc2: "(c, d) \<in> sc wit'"
+             and nin_sc1: "(c, d) \<notin> sc (incWit s)"
+             and nin_prev: "(c, d) \<notin> ?prev"
+             and nin_succ: "(c, d) \<notin> ?succ"
+          have d: "is_seq_cst d" "d \<in> actions0 pre'" "d \<noteq> c"
+            using cons2 in_sc2 by auto
+          have c:  "is_seq_cst c" "c \<in> actions0 pre'" "d \<noteq> c"
+            using cons2 in_sc2 by auto
+          have "c \<noteq> a"
+            proof
+              assume "c = a"
+              hence d2: "d \<in> incCommittedSet s" using d committed by simp
+              have "(b, d) \<in> sc wit'" 
+                using transE[OF transitive] b in_sc2 `c = a` by auto
+              hence "(b, d) \<in> sc (incWit s)" using b3 d2 wit by auto
+              hence "(c, d) \<in> ?succ" using d d2 `c = a` by auto
+              thus False using nin_succ by simp
+            qed
+          hence c2: "c \<in> incCommittedSet s" using c committed by auto
+          thus "d = a" 
+            using d committed in_sc2 nin_sc1 wit by auto
+          have bc_nin_sc: "(b, c) \<notin> sc wit'" using max c in_sc2 `d = a` by simp
+          have "(c, b) \<notin> sc (incWit s)" using nin_prev `d = a` c c2 by auto
+          hence "(c, b) \<notin> sc wit'" using b3 c2 wit by auto
+          thus "c = b" 
+            using cons2 bc_nin_sc b2 b3(2) c(1) c(2) by auto
+        qed
+      ultimately have "sc wit' = sc (incWit s) \<union> ?prev \<union> ?succ \<union> {(b, a)}" 
+        using b by auto        
+      thus ?thesis
+        using b b3 
+        unfolding addToTransitiveOrder_def scActionsSet_def
+        by auto
+    qed
+qed
+
+corollary step_sc:
+  assumes cons2:     "axsimpConsistentAlt pre' wit'"
+      and wit:       "incWit s = incWitRestrict wit' (incCommittedSet s)"
+      and committed: "actions0 pre' = insert a (incCommittedSet s)"
+      and a:         "a \<in> actions0 pre'" "a \<notin> incCommittedSet s"
+  shows              "if is_seq_cst a 
+                      then sc wit' [\<in>] monAddToSc pre a s 
+                      else sc wit' = sc (incWit s)"
+proof (cases "is_seq_cst a")
+  assume "is_seq_cst a"
+  thus ?thesis 
+    using step_sc_is_sc[OF cons2 wit committed] a by simp
+next
+  assume "\<not>is_seq_cst a"
+  thus ?thesis 
+    using step_sc_isnot_sc[OF cons2 wit committed] a by simp
+qed
+
+subsubsection {* lo-order *}
+
+lemma step_lo_not_lock_unlock:
+  assumes cons2:     "axsimpConsistentAlt pre' wit'"
+      and wit:       "incWit s = incWitRestrict wit' (incCommittedSet s)"
+      and committed: "actions0 pre' = insert a (incCommittedSet s)"
+      and a:         "a \<notin> incCommittedSet s \<and> \<not>is_lock a \<and> \<not>is_unlock a"
+  shows              "lo wit' = lo (incWit s)"
+proof (intro equalityI subsetI, auto)
+  fix b c
+  assume "(b, c) \<in> lo (incWit s)"
+  thus "(b, c) \<in> lo wit'" using wit by simp
+next
+  fix b c
+  assume in_lo: "(b, c) \<in> lo wit'"
+  have "(is_lock b \<or> is_unlock b)" "b \<in> actions0 pre'" 
+       "(is_lock c \<or> is_unlock c)" "c \<in> actions0 pre'"
+    using cons2 in_lo by auto
+  hence "b \<in> incCommittedSet s" "c \<in> incCommittedSet s"
+     using cons2 a in_lo committed by auto
+  thus "(b, c) \<in> lo (incWit s)"
+    using cons2 wit committed in_lo by auto
+qed
 
 
+lemma step_lo_lock_unlock:
+  assumes cons2:     "axsimpConsistentAlt pre' wit'"
+      and wit:       "incWit s = incWitRestrict wit' (incCommittedSet s)"
+      and committed: "actions0 pre' = insert a (incCommittedSet s)"
+      and a:         "a \<in> actions0 pre'" "a \<notin> incCommittedSet s"
+      and is_lo_ulo: "is_lock a \<or> is_unlock a"
+  shows              "lo wit' [\<in>] monAddToLo pre a s"
+(* TODO: this lemma is an almost-clone of step_sc_is_sc. *)
+unfolding monAddToLo_def
+proof -
+  let ?lo_list = "sameLocLocksUnlocks (incCommitted s) a"
+  let ?lo_set  = "sameLocLocksUnlocksSet (incCommitted s) a"
+  have "actions_respect_location_kinds (actions0 pre') (lk pre')"
+    using cons2 by auto
+  hence mutex: "is_at_mutex_location (lk pre') a"
+    unfolding actions_respect_location_kinds_def is_at_mutex_location_def
+    using a is_lo_ulo by (cases a) auto
+  show "lo wit' [\<in>] addToTransitiveOrder ?lo_list a (lo (incWit s))"
+    proof (cases "\<exists>b. (b, a) \<in> lo wit'")
+      assume max: "\<not> (\<exists>b. (b, a) \<in> lo wit')"
+      have "lo wit' = lo (incWit s) \<union> Pair a ` ?lo_set"
+        proof auto
+          fix c
+          assume "c \<in> sameLocLocksUnlocksSet (incCommitted s) a"
+          hence c: "c \<in> incCommittedSet s" 
+                   "loc_of a = loc_of c" 
+                   "is_lock c \<or> is_unlock c" 
+                   "c \<in> actions0 pre'"
+            using committed by auto
+          hence "a \<noteq> c" using a by auto
+          have "(c, a) \<notin> lo wit'" using max by auto
+          thus "(a, c) \<in> lo wit'"
+            using cons2 a(1) c is_lo_ulo `a \<noteq> c` mutex 
+            by (auto elim: locks_only_consistent_loE2_inv)
+          fix c
+        next
+          fix b c
+          assume "(b, c) \<in> lo (incWit s)"
+          thus "(b, c) \<in> lo wit'" using wit by simp
+        next
+          fix b c
+          assume in_lo: "(b, c) \<in> lo wit'"
+             and not_new: "(b, c) \<notin> Pair a ` ?lo_set"
+          have "c \<noteq> a" using in_lo max by auto
+          have c: "loc_of b = loc_of c" "is_lock c \<or> is_unlock c"
+                  "c \<in> actions0 pre'" "b \<in> actions0 pre'"
+            using cons2 in_lo by auto
+          hence "c \<in> incCommittedSet s"
+            using `c \<noteq> a` committed by auto
+          hence "b \<noteq> a \<or> loc_of c \<noteq> loc_of a"
+            using not_new
+            unfolding sameLocLocksUnlocksSet_def
+            using c by auto
+          hence "b \<noteq> a" using c by auto
+          hence "b \<in> incCommittedSet s"
+            using committed `b \<in> actions0 pre'` by auto          
+          thus "(b, c) \<in> lo (incWit s)" 
+            using wit in_lo `c \<in> incCommittedSet s` by auto
+        qed
+      thus ?thesis unfolding addToTransitiveOrder_def by auto
+    next
+      assume "\<exists>b'. (b', a) \<in> lo wit'"
+      then obtain b' where b': "(b', a) \<in> lo wit'" by fast
 
+      let ?lo_set2 = "{x. (x, a) \<in> lo wit'}"
+  
+      have "b' \<in> ?lo_set2" using b' by simp
+      hence non_empty: "?lo_set2 \<noteq> {}" by fast
+      hence "finite_prefixes (lo wit') (actions0 pre')"
+        using cons2 by auto
+      hence finite: "finite ?lo_set2"
+        unfolding finite_prefixes_def using a by fast
+      hence irreflexive: "irrefl (lo wit')"
+      and   transitive:  "trans (lo wit')"
+        using cons2 by auto 
+      hence isOrder: "isStrictPartialOrder (lo wit')" 
+        unfolding isStrictPartialOrder_def by simp
+      obtain b where b:   "b \<in> ?lo_set2"
+                 and max: "(\<forall>y. y \<in> ?lo_set2 \<longrightarrow> (b, y) \<notin> lo wit')"
+        using supremum_partial_order[OF finite non_empty isOrder] by auto
+      have b2: "b \<in> actions0 pre'" using b cons2 by auto
+      hence b3: "b \<in> incCommittedSet s" "b \<noteq> a" "loc_of b = loc_of a" 
+               "is_lock b \<or> is_unlock b" "is_at_mutex_location (lk pre') b"
+        using b cons2 unfolding committed by auto
+
+      let ?prev = "(\<lambda>c. (c, a)) ` {x \<in> ?lo_set. (x, b) \<in> lo (incWit s)}"
+      let ?succ = "(\<lambda>c. (a, c)) ` {x \<in> ?lo_set. (b, x) \<in> lo (incWit s)}"
+
+      have "lo (incWit s) \<subseteq> lo wit'" using wit by auto 
+      moreover have "?prev \<subseteq> lo wit'" 
+        proof clarify
+          fix c
+          assume "(c, b) \<in> lo (incWit s)"
+          hence "(c, b) \<in> lo wit'" using wit by auto
+          thus "(c, a) \<in> lo wit'" using transitive b transE by auto
+        qed
+      moreover have "?succ \<subseteq> lo wit'"
+        proof auto
+          fix c
+          assume sameLoc: "c \<in> sameLocLocksUnlocksSet (incCommitted s) a"
+          assume in_sc: "(b, c) \<in> lo (incWit s)"
+          hence c: "c \<in> actions0 pre'" 
+                   "c \<in> incCommittedSet s" 
+                   "loc_of a = loc_of c" 
+                   "is_lock c \<or> is_unlock c"
+            using cons2 wit a sameLoc by auto
+          have "(b, c) \<in> lo wit'" using in_sc wit by auto
+          hence "(c, a) \<notin> lo wit'" using max c by auto
+          thus "(a, c) \<in> lo wit'" 
+            using sameLoc cons2 c a is_lo_ulo mutex
+            by (auto elim: locks_only_consistent_loE2_inv)
+        qed
+      moreover have "lo wit' \<subseteq> lo (incWit s) \<union> {(b, a)} \<union> ?prev \<union> ?succ"
+        proof auto
+          fix c d
+          assume in_lo2: "(c, d) \<in> lo wit'"
+             and nin_lo1: "(c, d) \<notin> lo (incWit s)"
+             and nin_prev: "(c, d) \<notin> ?prev"
+             and nin_succ: "(c, d) \<notin> ?succ"
+          have d: "d \<in> actions0 pre'" "d \<noteq> c" 
+                  "loc_of c = loc_of d" "is_lock d \<or> is_unlock d"
+            using cons2 in_lo2 by auto
+          have c: "c \<in> actions0 pre'" "d \<noteq> c" 
+                  "loc_of c = loc_of d" "is_lock c \<or> is_unlock c"
+            using cons2 in_lo2 by auto
+          have "c \<noteq> a"
+            proof
+              assume "c = a"
+              hence d2: "d \<in> incCommittedSet s" using d committed by simp
+              have "(b, d) \<in> lo wit'" 
+                using transE[OF transitive] b in_lo2 `c = a` by auto
+              hence "(b, d) \<in> lo (incWit s)" using b3 d2 wit by auto
+              hence "(c, d) \<in> ?succ" 
+                unfolding sameLocLocksUnlocksSet_def
+                using d d2 `c = a` 
+                by auto
+              thus False using nin_succ by simp
+            qed
+          hence c2: "c \<in> incCommittedSet s" using c committed by auto
+          thus "d = a" 
+            using d committed in_lo2 nin_lo1 wit by auto
+          have bc_nin_lo: "(b, c) \<notin> lo wit'" using max c in_lo2 `d = a` by simp
+          have loc: "loc_of b = loc_of c" using b3 c `d = a` by auto
+          have "(c, b) \<notin> lo (incWit s)"
+            using nin_prev `d = a` c c2
+            unfolding sameLocLocksUnlocksSet_def 
+            by auto
+          hence "(c, b) \<notin> lo wit'" using b3 c2 wit by auto
+          thus "c = b" 
+            using cons2 bc_nin_lo b2 b3(4) b3(5) c(1) c(4) loc 
+            by (auto elim: locks_only_consistent_loE2_inv)
+        qed
+      ultimately have "lo wit' = lo (incWit s) \<union> ?prev \<union> ?succ \<union> {(b, a)}" 
+        using b by auto             
+      thus ?thesis
+        using b b3 
+        unfolding addToTransitiveOrder_def sameLocLocksUnlocksSet_def Let_def
+        by auto
+    qed
+qed
+
+subsubsection {* tot-order *}
+
+lemma step_tot:
+  assumes cons2: "axsimpConsistentAlt pre' wit'"
+      and wit:   "incWit s = incWitRestrict wit' (incCommittedSet s)"
+  shows          "tot wit' = tot (incWit s)"
+proof -
+  have "tot wit' = {}"
+    using cons2 by auto
+  thus "tot wit' = tot (incWit s)"
+    using wit by auto
+qed
+
+subsubsection {* Perform action *}
+
+lemma monPerformLoadCompleteness:
+  assumes cons2:      "axsimpConsistentAlt pre' wit'"
+      and wit:        "incWit s = incWitRestrict wit' (incCommittedSet s)"
+      and committed:  "actions0 pre' = insert a (incCommittedSet s)"
+      and downclosed: "downclosed (incCommittedSet s) (rf wit')"
+      and a:          "a \<in> actions0 pre'" "a \<notin> incCommittedSet s"
+      and a2:         "is_load a"
+  shows               "wit' [\<in>] monPerformLoad pre s a"
+proof -
+  have "\<not> is_write a" using a2 by (cases a) auto
+  hence mo: "mo wit' = mo (incWit s)" 
+    using step_mo_not_atomic_write[OF cons2 wit committed] a by simp
+  have rf: "rf wit' [\<in>] monAddToRfLoad pre a s"
+    using step_rf_load[OF cons2 downclosed wit committed] a a2 by simp
+  have sc: "if is_seq_cst a 
+            then sc wit' [\<in>] monAddToSc pre a s 
+            else sc wit' = sc (incWit s)"
+    using step_sc[OF cons2 wit committed] a by simp      
+  have "\<not>is_lock a \<and> \<not>is_unlock a" using a2 by (cases a) auto
+  hence lo: "lo wit' = lo (incWit s)" 
+    using step_lo_not_lock_unlock[OF cons2 wit committed] a by simp
+  have tot: "tot wit' = tot (incWit s)" 
+    using step_tot[OF cons2 wit] by simp
+  show ?thesis
+    unfolding monPerformLoad_def
+    using cons2 rf mo lo sc tot
+    apply auto
+    (* TODO: don't know why auto can't figure this out. *)
+    apply (intro exI[where x="sc wit'"])
+    by auto
+qed   
+
+lemma monPerformStoreCompleteness:
+  assumes cons2:         "axsimpConsistentAlt pre' wit'"
+      and wit:           "incWit s = incWitRestrict wit' (incCommittedSet s)"
+      and committed:     "actions0 pre' = insert a (incCommittedSet s)"
+      and downclosed_mo: "downclosed (incCommittedSet s) (mo wit')"
+      and downclosed_rf: "downclosed (incCommittedSet s) (rf wit')"
+      and lk:            "case loc_of a of None \<Rightarrow> true | Some v \<Rightarrow> (lk pre') v = (lk pre) v"
+      and a:             "a \<in> actions0 pre'" "a \<notin> incCommittedSet s"
+      and a2:            "is_store a"
+  shows                  "wit' [\<in>] monPerformStore pre s a"
+proof -
+  have mo: "if is_at_atomic_location (lk pre) a
+            then mo wit' [\<in>] monAddToMo pre a s 
+            else mo wit' = mo (incWit s)"
+    proof 
+      assume "is_at_atomic_location (lk pre) a"
+      hence loc: "is_at_atomic_location (lk pre') a"
+        unfolding is_at_atomic_location_def 
+        using lk
+        by (cases "loc_of a") auto
+      have "is_write a" using a2 by (cases a) auto
+      thus "mo wit' [\<in>] monAddToMo pre a s"
+        using loc step_mo_atomic_write[OF cons2 wit committed downclosed_mo] a a2
+        by simp
+    next
+      assume loc: "\<not>is_at_atomic_location (lk pre) a"
+      hence loc: "\<not>is_at_atomic_location (lk pre') a" 
+        unfolding is_at_atomic_location_def 
+        using lk
+        by (cases "loc_of a") auto
+      have "actions_respect_location_kinds (actions0 pre') (lk pre')"
+        using cons2 by auto
+      hence "is_at_non_atomic_location (lk pre') a"
+        unfolding actions_respect_location_kinds_def 
+        using loc a a2
+        unfolding is_at_atomic_location_def is_at_non_atomic_location_def
+        by (cases a) auto
+      thus "mo wit' = mo (incWit s)"
+        using loc step_mo_not_atomic_write[OF cons2 wit committed] by auto
+    qed      
+  have "\<not> is_read a" using a2 by (cases a) auto
+  hence rf: "rf wit' = rf (incWit s)" 
+    using step_rf_non_read[OF cons2 downclosed_rf wit committed] a by simp
+  have sc: "if is_seq_cst a 
+            then sc wit' [\<in>] monAddToSc pre a s 
+            else sc wit' = sc (incWit s)"
+    using step_sc[OF cons2 wit committed] a by simp             
+  have "\<not>is_lock a \<and> \<not>is_unlock a" using a2 by (cases a) auto
+  hence lo: "lo wit' = lo (incWit s)" 
+    using step_lo_not_lock_unlock[OF cons2 wit committed] a by simp
+  have tot: "tot wit' = tot (incWit s)" 
+    using step_tot[OF cons2 wit] by simp
+  show ?thesis
+    unfolding monPerformStore_def 
+    using cons2 rf mo lo sc tot
+    apply auto
+    (* TODO: don't know why auto can't figure this out. *)
+    apply (intro exI[where x="sc wit'"])
+    by auto
+qed   
+
+lemma monPerformRmwCompleteness:
+  assumes cons2:         "axsimpConsistentAlt pre' wit'"
+      and wit:           "incWit s = incWitRestrict wit' (incCommittedSet s)"
+      and committed:     "actions0 pre' = insert a (incCommittedSet s)"
+      and downclosed_mo: "downclosed (incCommittedSet s) (mo wit')"
+      and downclosed_rf: "downclosed (incCommittedSet s) (rf wit')"
+      and a:             "a \<in> actions0 pre'" "a \<notin> incCommittedSet s"
+      and a2:            "is_RMW a"
+  shows                  "wit' [\<in>] monPerformRmw pre s a"
+proof -
+  have loc: "is_at_atomic_location (lk pre') a"
+    using is_RMWE_location_kind[OF a2 a(1)] cons2 by auto
+  have "is_write a" using a2 by (cases a) auto
+  hence mo: "mo wit' [\<in>] monAddToMo pre a s"
+    using loc step_mo_atomic_write[OF cons2 wit committed downclosed_mo] a a2
+    by simp
+  have rf: "rf wit' [\<in>] monAddToRfRmw pre a s"
+    using step_rf_rmw[OF cons2 downclosed_rf downclosed_mo wit committed] a a2 by simp
+  have sc: "if is_seq_cst a 
+            then sc wit' [\<in>] monAddToSc pre a s 
+            else sc wit' = sc (incWit s)"
+    using step_sc[OF cons2 wit committed] a by simp             
+  have "\<not>is_lock a \<and> \<not>is_unlock a" using a2 by (cases a) auto
+  hence lo: "lo wit' = lo (incWit s)" 
+    using step_lo_not_lock_unlock[OF cons2 wit committed] a by simp
+  have tot: "tot wit' = tot (incWit s)" 
+    using step_tot[OF cons2 wit] by simp
+  show ?thesis
+    unfolding monPerformRmw_def 
+    using cons2 rf mo lo sc tot
+    apply simp
+    (* TODO: don't know why auto can't figure this out. *)
+    apply (intro exI[where x="sc wit'"])
+    apply auto
+    apply (intro exI[where x="rf wit'"])
+    defer
+    apply (intro exI[where x="rf wit'"])
+    by auto
+qed
+
+lemma monPerformLockCompleteness:
+  assumes cons2:         "axsimpConsistentAlt pre' wit'"
+      and wit:           "incWit s = incWitRestrict wit' (incCommittedSet s)"
+      and committed:     "actions0 pre' = insert a (incCommittedSet s)"
+      and downclosed_rf: "downclosed (incCommittedSet s) (rf wit')"
+      and a:             "a \<in> actions0 pre'" "a \<notin> incCommittedSet s"
+      and a2:            "is_lock a"
+  shows                  "wit' [\<in>] monPerformLock pre s a"
+proof -
+  have "\<not> is_write a" using a2 by (cases a) auto
+  hence mo: "mo wit' = mo (incWit s)" 
+    using step_mo_not_atomic_write[OF cons2 wit committed] a by simp
+  have "\<not> is_read a" using a2 by (cases a) auto
+  hence rf: "rf wit' = rf (incWit s)" 
+    using step_rf_non_read[OF cons2 downclosed_rf wit committed] a by simp
+  have "\<not> is_seq_cst a" using a2 by (cases a) auto
+  hence sc: "sc wit' = sc (incWit s)"
+    using step_sc_isnot_sc[OF cons2 wit committed] a by simp          
+  hence lo: "lo wit' [\<in>] monAddToLo pre a s" 
+    using step_lo_lock_unlock[OF cons2 wit committed] a a2 by simp
+  have tot: "tot wit' = tot (incWit s)" 
+    using step_tot[OF cons2 wit] by simp
+  show ?thesis
+    unfolding monPerformLock_def
+    using cons2 rf mo lo sc tot
+    by auto
+qed   
+
+lemma monPerformUnlockCompleteness:
+  assumes cons2:         "axsimpConsistentAlt pre' wit'"
+      and wit:           "incWit s = incWitRestrict wit' (incCommittedSet s)"
+      and committed:     "actions0 pre' = insert a (incCommittedSet s)"
+      and downclosed_rf: "downclosed (incCommittedSet s) (rf wit')"
+      and a:             "a \<in> actions0 pre'" "a \<notin> incCommittedSet s"
+      and a2:            "is_unlock a"
+  shows                  "wit' [\<in>] monPerformUnlock pre s a"
+proof -
+  have "\<not> is_write a" using a2 by (cases a) auto
+  hence mo: "mo wit' = mo (incWit s)" 
+    using step_mo_not_atomic_write[OF cons2 wit committed] a by simp
+  have "\<not> is_read a" using a2 by (cases a) auto
+  hence rf: "rf wit' = rf (incWit s)" 
+    using step_rf_non_read[OF cons2 downclosed_rf wit committed] a by simp
+  have "\<not> is_seq_cst a" using a2 by (cases a) auto
+  hence sc: "sc wit' = sc (incWit s)"
+    using step_sc_isnot_sc[OF cons2 wit committed] a by simp          
+  hence lo: "lo wit' [\<in>] monAddToLo pre a s" 
+    using step_lo_lock_unlock[OF cons2 wit committed] a a2 by simp
+  have tot: "tot wit' = tot (incWit s)" 
+    using step_tot[OF cons2 wit] by simp
+  show ?thesis
+    unfolding monPerformUnlock_def
+    using cons2 rf mo lo sc tot
+    by auto
+qed   
+
+lemma monPerformFenceCompleteness:
+  assumes cons2:         "axsimpConsistentAlt pre' wit'"
+      and wit:           "incWit s = incWitRestrict wit' (incCommittedSet s)"
+      and committed:     "actions0 pre' = insert a (incCommittedSet s)"
+      and downclosed_rf: "downclosed (incCommittedSet s) (rf wit')"
+      and a:             "a \<in> actions0 pre'" "a \<notin> incCommittedSet s"
+      and a2:            "is_fence a"
+  shows                  "wit' [\<in>] monPerformFence pre s a"
+proof -
+  have "\<not> is_write a" using a2 by (cases a) auto
+  hence mo: "mo wit' = mo (incWit s)" 
+    using step_mo_not_atomic_write[OF cons2 wit committed] a by simp
+  have "\<not> is_read a" using a2 by (cases a) auto
+  hence rf: "rf wit' = rf (incWit s)" 
+    using step_rf_non_read[OF cons2 downclosed_rf wit committed] a by simp
+  have sc: "if is_seq_cst a 
+            then sc wit' [\<in>] monAddToSc pre a s 
+            else sc wit' = sc (incWit s)"
+    using step_sc[OF cons2 wit committed] a by simp         
+  have "\<not>is_lock a \<and> \<not>is_unlock a" using a2 by (cases a) auto
+  hence lo: "lo wit' = lo (incWit s)" 
+    using step_lo_not_lock_unlock[OF cons2 wit committed] a by simp
+  have tot: "tot wit' = tot (incWit s)" 
+    using step_tot[OF cons2 wit] by simp
+  show ?thesis
+    unfolding monPerformFence_def
+    using cons2 rf mo lo sc tot
+    by auto
+qed     
+
+lemma ignoreActionCompleteness:
+  assumes cons2:         "axsimpConsistentAlt pre' wit'"
+      and wit:           "incWit s = incWitRestrict wit' (incCommittedSet s)"
+      and committed:     "actions0 pre' = insert a (incCommittedSet s)"
+      and downclosed_rf: "downclosed (incCommittedSet s) (rf wit')"
+      and a:             "a \<in> actions0 pre'" "a \<notin> incCommittedSet s"
+      and a2:            "\<not> is_write a" 
+                         "\<not> is_read a" 
+                         "\<not> is_seq_cst a" 
+                         "\<not> is_lock a" 
+                         "\<not> is_unlock a"
+  shows                  "wit' = incWit s"
+proof -
+  have mo: "mo wit' = mo (incWit s)" 
+    using step_mo_not_atomic_write[OF cons2 wit committed] a2 by simp
+  have rf: "rf wit' = rf (incWit s)" 
+    using step_rf_non_read[OF cons2 downclosed_rf wit committed] a a2 by simp
+  have sc: "sc wit' = sc (incWit s)"
+    using step_sc_isnot_sc[OF cons2 wit committed] a a2 by simp          
+  have lo: "lo wit' = lo (incWit s)" 
+    using step_lo_not_lock_unlock[OF cons2 wit committed] a a2 by simp
+  have tot: "tot wit' = tot (incWit s)" 
+    using step_tot[OF cons2 wit] by simp
+  show ?thesis
+    using cons2 rf mo lo sc tot
+    by auto
+qed
+
+lemma monPerformActionCompleteness:
+  assumes cons2:         "axsimpConsistentAlt pre' wit'"
+      and wit:           "incWit s = incWitRestrict wit' (incCommittedSet s)"
+      and committed:     "actions0 pre' = insert a (incCommittedSet s)"
+      and downclosed_rf: "downclosed (incCommittedSet s) (rf wit')"
+      and downclosed_mo: "downclosed (incCommittedSet s) (mo wit')"
+      and lk:            "case loc_of a of None \<Rightarrow> true | Some v \<Rightarrow> (lk pre') v = (lk pre) v"
+      and a:             "a \<in> actions0 pre'" "a \<notin> incCommittedSet s"
+  shows                  "wit' [\<in>] monPerformAction pre s a"
+proof (cases a)
+  case Load
+  thus ?thesis
+    unfolding monPerformAction_def
+    using monPerformLoadCompleteness[OF cons2 wit committed downclosed_rf a]
+    by auto
+next
+  case Store
+  thus ?thesis
+    unfolding monPerformAction_def
+    using monPerformStoreCompleteness[OF cons2 wit committed downclosed_mo downclosed_rf lk a]
+    by auto
+next
+  case RMW
+  thus ?thesis
+    unfolding monPerformAction_def
+    using monPerformRmwCompleteness[OF cons2 wit committed downclosed_mo downclosed_rf a]
+    by auto
+next
+  case Lock
+  thus ?thesis
+    unfolding monPerformAction_def
+    using monPerformLockCompleteness[OF cons2 wit committed downclosed_rf a] 
+    by auto
+next
+  case Unlock
+  thus ?thesis
+    unfolding monPerformAction_def
+    using monPerformUnlockCompleteness[OF cons2 wit committed downclosed_rf a] 
+    by auto
+next
+  case Fence
+  thus ?thesis
+    unfolding monPerformAction_def
+    using monPerformFenceCompleteness[OF cons2 wit committed downclosed_rf a] 
+    by auto
+next
+  case Blocked_rmw
+  thus ?thesis
+    unfolding monPerformAction_def
+    using ignoreActionCompleteness[OF cons2 wit committed downclosed_rf a]
+    by auto
+next
+  case Alloc
+  thus ?thesis
+    unfolding monPerformAction_def
+    using ignoreActionCompleteness[OF cons2 wit committed downclosed_rf a]
+    by auto
+next
+  case Dealloc
+  thus ?thesis
+    unfolding monPerformAction_def
+    using ignoreActionCompleteness[OF cons2 wit committed downclosed_rf a]
+    by auto
+qed
+
+subsubsection {* monStep, monTrace *}
+
+lemma monStepCompleteness:
+  assumes step:      "incStep pre s1 s2 a"
+      and finite:    "finite (actions0 pre)"
+      and invariant: "incCommittedSet s1 \<subseteq> actions0 pre"
+  shows              "(a, s2) [\<in>] monStep pre s1"
+proof -
+  let ?pre' = "preRestrict pre (incCommittedSet s2)"
+  have cons:      "axsimpConsistentAlt ?pre' (incWit s2)"
+   and a:         "a \<in> actions0 pre" "a \<notin> incCommittedSet s1"
+   and committed: "incCommitted s2 = a # (incCommitted s1)"
+   and wit:       "incWit s1 = incWitRestrict (incWit s2) (incCommittedSet s1)"
+   and order:     "respectsCom (actions0 pre) (incCommitted s1) (incComAlt ?pre' (incWit s2)) a"
+    using step unfolding incStep_def Let_def incToEx_def by auto
+  have committed2: "actions0 ?pre' = insert a (incCommittedSet s1)"
+    using committed a invariant by auto
+  have lk: "case loc_of a of 
+              None \<Rightarrow> True 
+            | Some v \<Rightarrow> lk (preRestrict pre (incCommittedSet s2)) v = lk pre v"
+    by (cases "loc_of a") simp_all
+  have a2: "a \<in> actions0 ?pre'"
+    using a committed by auto    
+  have downclosed_rf: "downclosed (incCommittedSet s1) (rf (incWit s2))"
+    unfolding downclosed_def
+    proof auto
+      fix x y
+      assume y:     "y \<in> incCommittedSet s1" 
+         and in_rf: "(x, y) \<in> rf (incWit s2)"
+      have "y \<in> actions0 ?pre'" using cons in_rf by blast
+      hence "y \<in> actions0 pre" by simp
+      hence "(a, y) \<notin> incComAlt ?pre' (incWit s2)"
+        using in_rf order y
+        unfolding respectsCom_def
+        by auto
+      hence "(a, y) \<notin> rf (incWit s2)"
+        unfolding incComAlt_def by auto
+      hence "x \<noteq> a" using in_rf by auto
+      have "x \<in> actions0 ?pre'" using cons in_rf by blast
+      hence "x \<in> incCommittedSet s2" by simp
+      thus "x \<in> incCommittedSet s1" using `x \<noteq> a` committed by simp
+    qed
+  have downclosed_mo: "downclosed (incCommittedSet s1) (mo (incWit s2))"
+    (* TODO: Clone of the proof of downclosed_rf. *)
+    unfolding downclosed_def
+    proof auto
+      fix x y
+      assume y:     "y \<in> incCommittedSet s1" 
+         and in_rf: "(x, y) \<in> mo (incWit s2)"
+      have "y \<in> actions0 ?pre'" using cons in_rf by blast
+      hence "y \<in> actions0 pre" by simp
+      hence "(a, y) \<notin> incComAlt ?pre' (incWit s2)"
+        using in_rf order y
+        unfolding respectsCom_def
+        by auto
+      hence "(a, y) \<notin> mo (incWit s2)"
+        unfolding incComAlt_def by auto
+      hence "x \<noteq> a" using in_rf by auto
+      have "x \<in> actions0 ?pre'" using cons in_rf by blast
+      hence "x \<in> incCommittedSet s2" by simp
+      thus "x \<in> incCommittedSet s1" using `x \<noteq> a` committed by simp
+    qed
+  have performAction: "incWit s2 [\<in>] monPerformAction pre s1 a"
+    using monPerformActionCompleteness[OF cons wit committed2 downclosed_rf 
+                                           downclosed_mo lk a2 a(2)] .
+  have cons2: "() [\<in>] monCheckConsistency (?pre', incWit s2, getRelations ?pre' (incWit s2))"
+    unfolding monCheckConsistency_def
+    using cons
+    by auto
+  show ?thesis
+    unfolding monStep_def Let_def
+    using wit committed performAction order a finite cons2
+    apply auto
+    apply (intro exI[where x=a])
+    by auto
+qed
+
+lemma monTraceCompleteness_aux:
+  assumes "incTrace pre r s"
+          "r = incInitialState pre"
+  shows   "monTrace pre r s"
+using assms
+proof induct
+  case (incReflexive pre s)
+  thus "monTrace pre s s"
+    using monReflexive by auto
+next
+  case (incStep pre x y z a)
+  have finite: "finite (actions0 pre)"
+    using incStep incTraceConsistency by auto
+  have inv: "incCommittedSet y \<subseteq> actions0 pre"
+    using incStep incTraceConsistency by auto
+  have "(a, z) [\<in>] monStep pre y" 
+    using monStepCompleteness[OF _ finite inv] incStep by auto
+  thus "monTrace pre x z"
+    using incStep monStep by auto
+qed
+
+corollary monTraceCompleteness:
+  assumes "incTrace pre (incInitialState pre) s"
+  shows   "monTrace pre (incInitialState pre) s"
+using assms monTraceCompleteness_aux by simp
+
+subsection {* Equivalence *}
+
+corollary monTraceEquivalence:
+  shows "  monTrace pre (incInitialState pre) s 
+         = incTrace pre (incInitialState pre) s"
+using monTraceSoundness monTraceCompleteness
+by metis
+
+lemma consistencyFromTraceEq:
+  assumes "\<And>pre s.  trace pre (incInitialState pre) s
+                   = trace' pre (incInitialState pre) s"
+  shows "consistencyFromTrace trace = consistencyFromTrace trace'"
+apply (intro ext, clarify)
+unfolding consistencyFromTrace.simps
+using assms
+by auto
+
+lemma monConsistentEquivalence_aux:  
+  shows "monConsistent = incConsistent"
+unfolding monConsistent_def incConsistent_def
+using consistencyFromTraceEq monTraceEquivalence
+by metis
+
+corollary monConsistentEquivalence:  
+  shows "  monConsistent (pre, wit, getRelations pre wit)
+         = (axConsistent (pre, wit, getRelations pre wit) \<and> finite (actions0 pre))"
+using monConsistentEquivalence_aux incConsistentEquivalence axsimpConsistentEq
+by metis
+
+(*<*)
 end
+(*>*)
